<|ref|>text<|/ref|><|det|>[[90, 66, 374, 84]]<|/det|>
c) Wir betrachten die Funktion 

<|ref|>equation<|/ref|><|det|>[[118, 95, 890, 117]]<|/det|>
\[f(x) = (x^3 - 1) \cdot (1 - x). \qquad (5)\]

<|ref|>text<|/ref|><|det|>[[118, 129, 390, 147]]<|/det|>
F端r die Ableitung erhalten wir 

<|ref|>equation<|/ref|><|det|>[[118, 157, 890, 216]]<|/det|>
\[\begin{aligned} f'(x) &= (x^3 - 1)' \cdot (1 - x) + (x^3 - 1) \cdot (1 - x)' = 3x^2 \cdot (1 - x) + (x^3 - 1) \cdot (-1) \\ &= 3x^2 - 3x^3 + 1 - x^3 = \frac{3x^2 - 4x^3 + 1}{x}. \end{aligned} \qquad (6)\]

<|ref|>text<|/ref|><|det|>[[90, 237, 374, 255]]<|/det|>
d) Wir betrachten die Funktion 

<|ref|>equation<|/ref|><|det|>[[118, 266, 890, 290]]<|/det|>
\[f(x) = (x^2 - x + 1)^2 = (x^2 - x + 1) \cdot (x^2 - x + 1). \qquad (7)\]

<|ref|>text<|/ref|><|det|>[[118, 302, 390, 320]]<|/det|>
F端r die Ableitung erhalten wir 

<|ref|>equation<|/ref|><|det|>[[118, 330, 890, 417]]<|/det|>
\[\begin{aligned} f'(x) &= (x^2 - x + 1)' \cdot (x^2 - x + 1) + (x^2 - x + 1) \cdot (x^2 - x +1)' \\ &= 2(x^2 - x + 1) \cdot (x^2 - x + 1)' = 2(x^2 - x + 1) \cdot (2x - 1) \\ &= 4x^3 - 4x^2 + 4x - 2x^2 + 2x - 2 = \frac{4x^3 - 6x^2 + 6x - 2}{x}. \end{aligned} \qquad (8)\]

<|ref|>text<|/ref|><|det|>[[90, 439, 374, 456]]<|/det|>
e) Wir betrachten die Funktion 

<|ref|>equation<|/ref|><|det|>[[118, 468, 890, 490]]<|/det|>
\[f(x) = (x + 1) \cdot \sqrt{x}. \qquad (9)\]

<|ref|>text<|/ref|><|det|>[[118, 502, 390, 520]]<|/det|>
F端r die Ableitung erhalten wir 

<|ref|>equation<|/ref|><|det|>[[118, 530, 890, 616]]<|/det|>
\[\begin{aligned} \frac{f'(x)}{x} &= (x + 1)' \cdot \sqrt{x} + (x + 1) \cdot (\sqrt{x})' = (1 + 0) \cdot \sqrt{x} + (x + 1) \cdot \frac{1}{2 \cdot \sqrt{x}} = \sqrt{x} + \frac{x + 1}{2 \cdot \sqrt{x}} \\ &= \frac{2 \cdot \sqrt{x} \cdot \sqrt{x}}{2 \cdot \sqrt{x}} + \frac{x + 1}{2 \cdot \sqrt{x}} = \frac{2 \cdot x + x + 1}{2 \cdot \sqrt{x}} = \frac{3x + 1}{2 \cdot \sqrt{x}}. \end{aligned} \qquad (10)\]

<|ref|>text<|/ref|><|det|>[[90, 636, 374, 654]]<|/det|>
f) Wir betrachten die Funktion 

<|ref|>equation<|/ref|><|det|>[[118, 665, 890, 700]]<|/det|>
\[f(x) = (x + 1) \cdot \frac{1}{x}. \qquad (11)\]

<|ref|>text<|/ref|><|det|>[[118, 710, 390, 728]]<|/det|>
F端r die Ableitung erhalten wir 

<|ref|>equation<|/ref|><|det|>[[118, 738, 890, 823]]<|/det|>
\[\begin{aligned} \frac{f'(x)}{x} &= (x +1)' \cdot \frac{1}{x} + (x+1) \cdot \left(\frac{1}{x}\right)' = (1+0) \cdot \frac{1}{x} + (x+1) \cdot (-1) \cdot \frac{1}{x^2} = \frac{1}{x} - \frac{x+1}{x^2} \\ &= \frac{x}{x^2} - \frac{x+1}{x^2} = \frac{x-x-1}{x^2} = \frac{0-1}{x^2} = -\frac{1}{x^2}. \end{aligned} \qquad (12)\]