<|ref|>text<|/ref|><|det|>[[118, 66, 494, 85]]<|/det|>
wobei \(c \in \mathbb{R}\) beliebig gewählt werden kann. 

<|ref|>text<|/ref|><|det|>[[90, 92, 240, 110]]<|/det|>
c) Wir erhalten 

<|ref|>equation<|/ref|><|det|>[[118, 119, 888, 170]]<|/det|>
\[f(x) = 2x \Rightarrow \begin{cases} f'(x) = 2 \\ F(x) = x^2 + c, \end{cases} \quad (47)\]

<|ref|>text<|/ref|><|det|>[[118, 186, 494, 205]]<|/det|>
wobei \(c \in \mathbb{R}\) beliebig gewählt werden kann, 

<|ref|>text<|/ref|><|det|>[[90, 212, 240, 230]]<|/det|>
d) Wir erhalten 

<|ref|>equation<|/ref|><|det|>[[118, 239, 888, 301]]<|/det|>
\[f(x) = x \Rightarrow \begin{cases} f'(x) = 1 \\ F(x) = \frac{1}{2}x^2 + c, \end{cases} \quad (48)\]

<|ref|>text<|/ref|><|det|>[[118, 316, 494, 334]]<|/det|>
wobei \(c \in \mathbb{R}\) beliebig gewählt werden kann 

<|ref|>text<|/ref|><|det|>[[90, 342, 240, 360]]<|/det|>
e) Wir erhalten 

<|ref|>equation<|/ref|><|det|>[[118, 369, 888, 430]]<|/det|>
\[f(x) = 3x \Rightarrow \begin{cases} f'(x) = 3 \\ F(x) = \frac{3}{2}x^2 + c, \end{cases} \quad (49)\]

<|ref|>text<|/ref|><|det|>[[118, 446, 494, 464]]<|/det|>
wobei \(c \in \mathbb{R}\) beliebig gewählt werden kann: 

<|ref|>text<|/ref|><|det|>[[90, 472, 240, 490]]<|/det|>
f) Wir erhalten 

<|ref|>equation<|/ref|><|det|>[[118, 499, 888, 561]]<|/det|>
\[f(x) = x^2 \Rightarrow \begin{cases} f'(x) = 2x^{2-1} = 2x \\ F(x) = \frac{1}{2+1}x^{2+1} + c = \frac{1}{3}x^3 + c, \end{cases} \quad (50)\]

<|ref|>text<|/ref|><|det|>[[118, 577, 494, 595]]<|/det|>
wobei \(c \in \mathbb{R}\) beliebig gewählt werden kann; 

<|ref|>text<|/ref|><|det|>[[90, 603, 273, 621]]<|/det|>
g) Für die Funktion 

<|ref|>equation<|/ref|><|det|>[[118, 631, 888, 652]]<|/det|>
\[f(x) = 3x^2 + 2 \quad (51)\]

<|ref|>text<|/ref|><|det|>[[118, 664, 230, 681]]<|/det|>
erhalten wir 

<|ref|>equation<|/ref|><|det|>[[118, 692, 888, 714]]<|/det|>
\[\frac{f'(x)}{x} = 3 \cdot 2 \cdot x^{2-1} + 0 = \frac{6x}{x} \quad (52)\]

<|ref|>equation<|/ref|><|det|>[[118, 728, 888, 764]]<|/det|>
\[\frac{F(x)}{x} = 3 \cdot \frac{1}{2+1}x^{2+1} + 2x + c = \frac{3}{3}x^3 + 2x + c = \frac{x^3 + 2x + c}{x} \quad (53)\]

<|ref|>text<|/ref|><|det|>[[118, 775, 494, 792]]<|/det|>
wobei \(c \in \mathbb{R}\) beliebig gewählt werden kann- 

<|ref|>text<|/ref|><|det|>[[90, 801, 273, 819]]<|/det|>
h) Für die Funktion 

<|ref|>equation<|/ref|><|det|>[[118, 829, 888, 850]]<|/det|>
\[f(x) = 6x^3 - 4x + 1 \quad (54)\]

<|ref|>text<|/ref|><|det|>[[118, 861, 230, 878]]<|/det|>
erhalten wir 

<|ref|>equation<|/ref|><|det|>[[118, 888, 888, 911]]<|/det|>
\[\frac{f'(x)}{x} = 6x^3 - 4x + 1 = 6 \cdot 3 \cdot x^{3-1} - 4 + 0 = \frac{18x^2 - 4}{x} \quad (55)\]