<|ref|>text<|/ref|><|det|>[[123, 66, 281, 85]]<|/det|>
f) Allgemein gilt 

<|ref|>equation<|/ref|><|det|>[[149, 96, 920, 134]]<|/det|>
\[ \frac{f(x-1)}{a} = a^{x-1} = \frac{a^x}{a^1} = \frac{f(x)}{a}. \qquad (25) \]

<|ref|>text<|/ref|><|det|>[[149, 149, 627, 168]]<|/det|>
Als Beispiel w채hlen wir \(a = 5\) und \(x = 3\). Wir erhalten 

<|ref|>equation<|/ref|><|det|>[[184, 179, 920, 198]]<|/det|>
\[ f(3) = 5^3 = 125 \qquad (26) \]

<|ref|>equation<|/ref|><|det|>[[149, 207, 920, 247]]<|/det|>
\[ \frac{f(3-1)}{5} = f(2) = 5^2 = 25 = \frac{125}{5} = \frac{f(3)}{5}. \qquad (27) \]

<|ref|>text<|/ref|><|det|>[[123, 264, 281, 283]]<|/det|>
g) Allgemein gilt 

<|ref|>equation<|/ref|><|det|>[[149, 293, 920, 315]]<|/det|>
\[ \frac{f(x+y)}{a} = a^{x+y} = a^x \cdot a^y = f(x) \cdot f(y). \qquad (28) \]

<|ref|>text<|/ref|><|det|>[[149, 332, 686, 351]]<|/det|>
Als Beispiel w채hlen wir \(a = 2\), \(x = 3\) und \(y = 5\). Wir erhalten 

<|ref|>equation<|/ref|><|det|>[[184, 362, 920, 381]]<|/det|>
\[ f(3) = 2^3 = 8 \qquad (29) \]

<|ref|>equation<|/ref|><|det|>[[184, 390, 920, 409]]<|/det|>
\[ f(5) = 2^5 = 32 \qquad (30) \]

<|ref|>equation<|/ref|><|det|>[[149, 416, 920, 440]]<|/det|>
\[ \frac{f(3+5)}{a} = f(8) = 2^8 = 256 = 8 \cdot 32 = f(3) \cdot f(5). \qquad (31) \]

<|ref|>text<|/ref|><|det|>[[123, 459, 281, 477]]<|/det|>
h) Allgemein gilt 

<|ref|>equation<|/ref|><|det|>[[149, 488, 920, 528]]<|/det|>
\[ \frac{f(x-y)}{a^y} = a^{x-y} = \frac{a^x}{a^y} = \frac{f(x)}{f(y)}. \qquad (32) \]

<|ref|>text<|/ref|><|det|>[[149, 545, 686, 563]]<|/det|>
Als Beispiel w채hlen wir \(a = 2\), \(x = 3\), und \(y = 5\). Wir erhalten 

<|ref|>equation<|/ref|><|det|>[[184, 575, 920, 593]]<|/det|>
\[ f(3) = 2^3 = 8 \qquad (33) \]

<|ref|>equation<|/ref|><|det|>[[184, 602, 920, 621]]<|/det|>
\[ f(5) = 2^5 = 32 \qquad (34) \]

<|ref|>equation<|/ref|><|det|>[[149, 630, 920, 670]]<|/det|>
\[ \frac{f(3-5)}{4} = f(-2) = 2^{-2} = \frac{1}{4} = \frac{8}{32} = \frac{f(3)}{f(5)}. \qquad (35) \]

<|ref|>text<|/ref|><|det|>[[123, 690, 281, 709]]<|/det|>
i) Allgemein gilt 

<|ref|>equation<|/ref|><|det|>[[149, 718, 920, 743]]<|/det|>
\[ \frac{f(x \cdot y)}{a} = a^{x \cdot y} = (a^x)^y = (f(x))^y = (f(y))^x. \qquad (36) \]

<|ref|>text<|/ref|><|det|>[[149, 760, 686, 779]]<|/det|>
Als Beispiel w채hlen wir \(a = 2\), \(x = 3 \), und \(y = 5\). Wir erhalten 

<|ref|>equation<|/ref|><|det|>[[179, 790, 920, 808]]<|/det|>
\[ f(3) = 2^3 = 8 \qquad (37) \]

<|ref|>equation<|/ref|><|det|>[[179, 817, 920, 836]]<|/det|>
\[ f(5) = 2^5 = 32 \qquad (38) \]

<|ref|>equation<|/ref|><|det|>[[149, 845, 920, 875]]<|/det|>
\[ \frac{f(3 \cdot 5)}{a} = f(15) = 2^{15} = 32^{768} = 8^5 = (f(3))^5 \qquad (39) \]

<|ref|>equation<|/ref|><|det|>[[149, 884, 920, 911]]<|/det|>
\[ \frac{f(3 \cdot 5)}{a} = f(5) = 2^{15} = 32^{768} = 32^3 = (f(5))^3. \qquad (40) \]