<|ref|>text<|/ref|><|det|>[[89, 66, 238, 84]]<|/det|>
e) Wir erhalten 

<|ref|>equation<|/ref|><|det|>[[117, 95, 816, 180]]<|/det|>
\[
\begin{align*}
F(x) &= \int 3^{2+x} dx = \int 3^2 \cdot 3^x dx = 9 \int 3^x dx = 9 \cdot \frac{1}{\ln(3)} \cdot 3^x + c = \frac{9}{\ln(3)} \cdot 3^x + c \\
&= \frac{1}{\ln(3)} \cdot 3^{2+x} + c.
\end{align*}
\]

<|ref|>text<|/ref|><|det|>[[89, 201, 238, 219]]<|/det|>
f) Wir erhalten 

<|ref|>equation<|/ref|><|det|>[[117, 230, 880, 320]]<|/det|>
\[
\begin{align*}
F(x) &= \int \frac{1}{3^{x-2}} dx = \int \frac{1}{3^x \cdot 3^{-2}} dx = \frac{1}{3^{-2}} \int \frac{1}{3^x} dx = \frac{1}{3^{-2}} \int \left(\frac{1}{3}\right)^x dx \\
&= \frac{1}{3^{-2}} \cdot \frac{1}{\ln\left(\frac{1}{3}\right)} \cdot \left(\frac{1}{3}\right)^x + c = \frac{1}{3^{-2}} \cdot \frac{1}{-\ln(3)} \cdot \frac{1}{3^x} + c = -\frac{1}{\ln(3)} \cdot \frac{1}{3^{x-2}} + c.
\end{align*}
\]