<|ref|>text<|/ref|><|det|>[[88, 66, 184, 85]]<|/det|>
d) Es gilt 

<|ref|>equation<|/ref|><|det|>[[118, 95, 888, 120]]<|/det|>
\[
\frac{f'(x)}{2} = 2 \cdot 16 \cdot x^{16-1} - 7 \cdot 2 \cdot x^{2-1} + 3 \cdot 10 \cdot x^{10-1} = 32x^{15} - 14x + 30x^9. \tag{31}
\]

<|ref|>text<|/ref|><|det|>[[88, 140, 184, 158]]<|/det|>
e) Es gilt 

<|ref|>equation<|/ref|><|det|>[[118, 169, 888, 194]]<|/det|>
\[
\frac{f'(x)}{2} = 2 \cdot x^{2-1} + 1 \cdot y + 0 = 2x + y. \tag{32}
\]

<|ref|>text<|/ref|><|det|>[[88, 214, 370, 232]]<|/det|>
f) Wir betrachten die Funktion 

<|ref|>equation<|/ref|><|det|>[[118, 242, 888, 278]]<|/det|>
\[
f(t) = \frac{1}{t} + t^{\frac{1}{2}}s^{-\frac{1}{2}} - \frac{1}{s} = t^{-1} + t^{\frac{1}{2}}s^{-\frac{1}{2}} - s. \tag{33}
\]

<|ref|>text<|/ref|><|det|>[[118, 287, 184, 305]]<|/det|>
Es gilt 

<|ref|>equation<|/ref|><|det|>[[118, 315, 888, 352]]<|/det|>
\[
\frac{\dot{f}(t)}{2} = (-1) \cdot t^{-1-1} + \frac{1}{2} \cdot t^{\frac{1}{2}-1} \cdot s^{-\frac{1}{2}} - 0 = -t^{-2} + \frac{1}{2} \cdot t^{-\frac{1}{2}}s^{-\frac{1}{2}}. \quad (34)
\]

<|ref|>text<|/ref|><|det|>[[88, 372, 370, 390]]<|/det|>
g) Wir betrachten die Funktion 

<|ref|>equation<|/ref|><|det|>[[118, 400, 888, 435]]<|/det|>
\[
f(s) = \frac{1}{t} + t^{\frac{1}{2}}s^{-1} - s^{-1}. \tag{35}
\]

<|ref|>text<|/ref|><|det|>[[118, 444, 184, 462]]<|/det|>
Es gilt 

<|ref|>equation<|/ref|><|det|>[[118, 472, 888, 510]]<|/det|>
\[
\frac{f'(s)}{2} = 0 + t^{\frac{1}{2}} \cdot \left(-\frac{1}{2}\right) \cdot s^{-\frac{1}{2}-1} - (-1) \cdot s^{-1-1} = -\frac{1}{2} \cdot t^{\frac{1}{2}}s^{-\frac{3}{2}} + s^{-2}. \quad (36)
\]

<|ref|>text<|/ref|><|det|>[[88, 531, 370, 549]]<|/det|>
h) Wir betrachten die Funktion 

<|ref|>equation<|/ref|><|det|>[[118, 560, 888, 585]]<|/det|>
\[
f(x) = 2 \cdot (x - 1)^2 = 2 \cdot (x^2 - 2x + 1). \tag{37}
\]

<|ref|>text<|/ref|><|det|>[[118, 595, 184, 613]]<|/det|>
Es gilt 

<|ref|>equation<|/ref|><|det|>[[118, 624, 888, 650]]<|/det|>
\[
\frac{f'(x)}{2} = 2 \cdot (2 \cdot x^{2-1} - 2 + 0) = 2 \cdot (2x - 2) = 4x - 4. \tag{38}
\]

<|ref|>text<|/ref|><|det|>[[88, 669, 370, 687]]<|/det|>
i) Wir betrachten die Funktion 

<|ref|>equation<|/ref|><|det|>[[118, 698, 888, 723]]<|/det|>
\[
f(y) = (x - y)^3 = x^3 - 3x^2y + 3xy^2 - y^3. \tag{39}
\]

<|ref|>text<|/ref|><|det|>[[118, 733, 184, 751]]<|/det|>
Es gilt 

<|ref|>equation<|/ref|><|det|>[[118, 761, 888, 820]]<|/det|>
\[
\begin{align*}
f'(y) &= 0 - 3x^2 \cdot 1 + 3x \cdot 2 \cdot y^{2-1} - 3 \cdot y^{3-1} = -3x^2 + 6xy - 3y^2 = -3 \cdot (x^2 - 2xy + y^2) \\
&= -3 \cdot (x - y)^2.
\end{align*}
\]