<|ref|>text<|/ref|><|det|>[[118, 66, 231, 83]]<|/det|>
erhalten wir 

<|ref|>equation<|/ref|><|det|>[[118, 90, 888, 131]]<|/det|>
\[ \frac{f'(x)}{2} = \frac{1}{2} \cdot x^{\frac{1}{2} - 1} = \frac{1}{2} x^{-\frac{1}{2}} = \frac{1}{2} \cdot \frac{1}{x^{\frac{1}{2}}} = \frac{1}{2 \sqrt{x}} \qquad (66) \]

<|ref|>equation<|/ref|><|det|>[[118, 144, 888, 185]]<|/det|>
\[ \frac{F(x)}{\frac{1}{2} + 1} = \frac{1}{\frac{1}{2} + 1} x^{\frac{1}{2} + 1} + c = \frac{1}{\frac{3}{2}} x^{\frac{3}{2}} + c = \frac{2}{3} \sqrt{x^3} + c, \qquad (67) \]

<|ref|>text<|/ref|><|det|>[[118, 199, 491, 217]]<|/det|>
wobei \(c \in \mathbb{R}\) beliebig gewählt werden kann. 

<|ref|>text<|/ref|><|det|>[[92, 225, 272, 243]]<|/det|>
1) Für die Funktion 

<|ref|>equation<|/ref|><|det|>[[118, 255, 888, 295]]<|/det|>
\[ f(x) = \sqrt{\frac{1}{x}} - 1 = \sqrt{x^{-1}} - 1 = (x^{-1})^{\frac{1}{2}} - 1 = x^{-1 \cdot \frac{1}{2}} - 1 = x^{-\frac{1}{2}} - 1 \qquad (68) \]

<|ref|>text<|/ref|><|det|>[[118, 305, 231, 321]]<|/det|>
erhalten wir 

<|ref|>equation<|/ref|><|det|>[[118, 330, 888, 370]]<|/det|>
\[ \frac{f'(x)}{-1} = -\frac{1}{2} \cdot x^{-\frac{1}{2} - 1} - 0 = -\frac{1}{2} x^{-\frac{3}{2}} = -\frac{1}{2} \cdot \frac{1}{x^{\frac{3}{2}}} = -\frac{1}{2 \sqrt{x^3}} \qquad (69) \]

<|ref|>equation<|/ref|><|det|>[[118, 383, 888, 422]]<|/det|>
\[ \frac{F(x)}{-\frac{1}{2} + 1} = \frac{1}{-\frac{1}{2} + 1} x^{-\frac{1}{2} + 1} - x + c = \frac{1}{2} x^{\frac{1}{2}} - x + c = 2 \sqrt{x} - x + c, \qquad (70) \]

<|ref|>text<|/ref|><|det|>[[118, 432, 491, 449]]<|/det|>
wobei \(c \in \mathbb{R}\) beliebig gewählt werden kann