<|ref|>text<|/ref|><|det|>[[89, 65, 576, 85]]<|/det|>
e) Wir skizzieren die Fläche I in einem x-y-Diagramm. 

<|ref|>image<|/ref|><|det|>[[191, 97, 819, 437]]<|/det|>
 

<|ref|>text<|/ref|><|det|>[[117, 449, 411, 468]]<|/det|>
Offensichtlich muss gelten \(I > 0\). 

<|ref|>equation<|/ref|><|det|>[[117, 477, 885, 523]]<|/det|>
\[
\underline{I} = \int_{0}^{3} 2^x \, dx = \frac{1}{\ln(2)} \cdot \left[ 2^x \right]_{0}^{3} = \frac{1}{\ln(2)} \cdot \left( 2^3 - 2^0 \right) = \frac{1}{\ln(2)} \cdot (8 - 1) = \frac{7}{\ln(2)}. \quad (17)
\]

<|ref|>text<|/ref|><|det|>[[89, 542, 576, 561]]<|/det|>
f) Wir skizzieren die Fläche I in einem x-y-Diagramm. 

  

<|ref|>image<|/ref|><|det|>[[139, 572, 870, 727]]<|/det|>
 

<|ref|>text<|/ref|><|det|>[[117, 740, 411, 759]]<|/det|>
Offensichtlich muss gelten \(I > 0\). 

<|ref|>equation
\[
\underline{I} = \int_{-4}^{0} 3^x \, dx = \frac{1}{\ln(3)} \cdot \left[ 3^x \right]_{-4}^{0} = \frac{1}{\ln(3)} \cdot \left( 3^0 - 3^{-4} \right) = \frac{1}{\ln(3)} \cdot \left( 1 - \frac{1}{3^4} \right)
\]