f) Allgemein gilt

$$
\underline{\underline{f(x-1)}}=a^{x-1}=\frac{a^{x}}{a^{1}}=\underline{\frac{f(x)}{a}}
$$

Als Beispiel w채hlen wir $a=5$ und $x=3$. Wir erhalten

$$
\begin{aligned}
f(3) & =5^{3}=125 \\
\underline{\underline{f(3-1)}} & =f(2)=5^{2}=25=\frac{125}{5}=\underline{\underline{\frac{f(3)}{5}}}
\end{aligned}
$$

g) Allgemein gilt

$$
\underline{\underline{f(x+y)}}=a^{x+y}=a^{x} \cdot a^{y}=\underline{\underline{f(x) \cdot f(y)}}
$$

Als Beispiel w채hlen wir $a=2, x=3$ und $y=5$. Wir erhalten

$$
\begin{aligned}
f(3) & =2^{3}=8 \\
f(5) & =2^{5}=32 \\
\underline{\underline{f(3+5)}} & =f(8)=2^{8}=256=8 \cdot 32=\underline{\underline{f(3) \cdot f(5)}}
\end{aligned}
$$

h) Allgemein gilt

$$
\underline{\underline{f(x-y)}}=a^{x-y}=\frac{a^{x}}{a^{y}}=\frac{f(x)}{\underline{\underline{f(y)}}}
$$

Als Beispiel w채hlen wir $a=2, x=3$ und $y=5$. Wir erhalten

$$
\begin{aligned}
f(3) & =2^{3}=8 \\
f(5) & =2^{5}=32 \\
\underline{\underline{f(3-5)}} & =f(-2)=2^{-2}=\frac{1}{4}=\frac{8}{32}=\underline{\underline{f(3)}} \\
\underline{\underline{(5)}}
\end{aligned}
$$

i) Allgemein gilt

$$
\underline{\underline{f(x \cdot y)}}=a^{x \cdot y}=\left(a^{x}\right)^{y}=\underline{\underline{(f(x))^{y}=(f(y))^{x}}}
$$

Als Beispiel w채hlen wir $a=2, x=3$ und $y=5$. Wir erhalten

$$
\begin{aligned}
f(3) & =2^{3}=8 \\
f(5) & =2^{5}=32 \\
\underline{\underline{f(3 \cdot 5)}}=f(15) & =2^{15}=32^{\prime} 768=8^{5}=\underline{\underline{(f(3))^{5}}} \\
\underline{\underline{f(3 \cdot 5)}}=f(15) & =2^{15}=32^{\prime} 768=32^{3}=\underline{\underline{(f(5))^{3}}}
\end{aligned}
$$