<|ref|>sub_title<|/ref|><|det|>[[25, 12, 519, 60]]<|/det|>
# Additionstheoreme 

<|ref|>text<|/ref|><|det|>[[48, 90, 207, 118]]<|/det|>
α, β ∈ ℝ 

<|ref|>text<|/ref|><|det|>[[25, 127, 680, 159]]<|/det|>
a) sin (α ± β) = sin α · cos β ± sinβ · cos α 

<|ref|>text<|/ref|><|det|>[[25, 167, 675, 199]]<|/det|>
b) cos (α ± β) = cos α · cosβ ± sinα · sinβ 

<|ref|>text<|/ref|><|det|>[[100, 207, 732, 240]]<|/det|>
Beweis: bekannt: cos α = sin (α + π/2) 

<|ref|>equation<|/ref|><|det|>[[240, 245, 710, 277]]<|/det|>
\[
\cos(\alpha \pm \beta) = \sin(\alpha \pm \beta + \frac{\pi}{2})
\]

<|ref|>equation<|/ref|><|det|>[[430, 280, 673, 312]]<|/det|>
\[
= \sin(\alpha + \frac{\pi}{2} \pm \beta)
\]

<|ref|>text<|/ref|><|det|>[[160, 320, 970, 365]]<|/det|>
mit α): = \(\frac{\sin(\alpha + \frac{\pi}{2}) \cdot \cos \beta \pm \sin \beta \cdot \cos(\alpha + \frac{\pi}{2})}{\cos \alpha}\) 

<|ref|>equation<|/ref|><|det|>[[430, 360, 957, 383]]<|/det|>
\[
= \cos \alpha \cdot \cos \beta \pm \sin \beta \cdot (-\sin \alpha)
\]

<|ref|>equation<|/ref|><|det|>[[430, 390, 848, 413]]<|/det|>
\[
= \cos \alpha \cdot \cos \beta \mp \sin \beta \cdot \sin \alpha
\]

<|ref|>text<|/ref|><|det|>[[25, 490, 460, 528]]<|/det|>
c) tan(α ± β) = \(\frac{\tan\alpha \pm \tan\beta}{1 \pm \tan\alpha \cdot \tan\beta}\) 

<|ref|>text<|/ref|><|det|>[[25, 548, 460, 586]]<|/det|>
d) cot(α ± β) = \(\frac{\cot\alpha \cdot \cot\beta \mp 1}{\cot\beta \pm \cot\alpha}\) 

<|ref|>text<|/ref|><|det|>[[25, 616, 680, 644]]<|/det|>
Vereinfachung trigonometrischer Funktionen, 

<|ref|>text<|/ref|><|det|>[[45, 653, 580, 682]]<|/det|>
die Argumente n: α (n ∈ N) besitzen 

<|ref|>text<|/ref|><|det|>[[52, 692, 650, 800]]<|/det|>
° sin (2α) = sin (α + α)
= sin α · cos α + sin α · cos α
= 2 · sin α · cos α 

<|ref|>text<|/ref|><|det|>[[52, 830, 625, 933]]<|/det|>
° cos (2α) = cos (α + α)
= cos α · cosβ - sin α · sin α
= cos² α - sin² α