<|ref|>text<|/ref|><|det|>[[20, 10, 460, 45]]<|/det|>
Bsp : a) \(\vec{v} = \begin{pmatrix} 1 \\ 0 \end{pmatrix}\) \(\vec{w} = \begin{pmatrix} 0 \\ 1 \end{pmatrix}\) 

<|ref|>equation<|/ref|><|det|>[[198, 66, 590, 96]]<|/det|>
bestimme \(\alpha\) zwischen \(\vec{v}\) & \(\vec{w}\)

<|ref|>equation<|/ref|><|det|>[[198, 99, 800, 188]]<|/det|>
\[ \begin{aligned} \alpha &= \cos^{-1}\left(\frac{\langle\vec{v}, \vec{w}\rangle}{\|\vec{v}\| \|\vec{w}\|}\right) = \cos^{-1}\left(\frac{1 \cdot 0 + 1 \cdot 1 + 0 \cdot 1}{\sqrt{1^2 + 1^2 + 0^2} \cdot \sqrt{0^2 + 1^2 + 1^2}}\right) \\ &= \cos^{-1}\left(\frac{1}{\sqrt{2} \cdot \sqrt{2}}\right) = \cos^{-1}\left(\frac{1}{2}\right) = 60^\circ = \frac{\pi}{3} \end{aligned} \]

<|ref|>text<|/ref|><|det|>[[130, 201, 626, 240]]<|/det|>
b) \(\vec{v} = \begin{pmatrix} \frac{2}{3} \\ -\frac{1}{4} \end{pmatrix}\) \(\vec{w} = \begin{pmatrix} \frac{1}{2} \\ \frac{1}{4} \end{pmatrix}\) \(c \in \mathbb{R}\) 

<|ref|>equation<|/ref|><|det|>[[198, 260, 490, 291]]<|/det|>
\(\vec{v} \perp \vec{w} : \text{was ist } c^2\)

<|ref|>equation<|/ref|><|det|>[[210, 301, 380, 327]]<|/det|>
\(\langle\vec{v}, \vec{w}\rangle = 0\)

<|ref|>equation<|/ref|><|det|>[[222, 330, 570, 370]]<|/det|>
\(2 \cdot 1 + 3 \cdot 2 + (-4) \cdot c = 0\)

<|ref|>equation<|/ref|><|det|>[[333, 380, 699, 410]]<|/det|>
\(8 - 4 \cdot c = 0 \quad | + 4c\)

<|ref|>equation<|/ref|><|det|>[[456, 420, 685, 450]]<|/det|>
\(8 = 4c \quad | : 4\)

<|ref|>equation<|/ref|><|det|>[[456, 462, 567, 491]]<|/det|>
\(c = 2\)

<|ref|>text<|/ref|><|det|>[[130, 519, 840, 550]]<|/det|>
c) Dreieck mit \(A(1; 4; -2)\), \(B(3; 1; 0)\), \(C(-1; 1; 2)\) 

<|ref|>text<|/ref|><|det|>[[198, 558, 960, 585]]<|/det|>
zu bestimmen: Seitengang des Dreiecks und Innenwinkel 

<|ref|>equation<|/ref|><|det|>[[210, 583, 870, 616]]<|/det|>
\(\overrightarrow{AB} = \overrightarrow{B-A} = \begin{pmatrix} \frac{3}{2} \\ -\frac{1}{2} \end{pmatrix} - \begin{pmatrix} \frac{1}{2} \\ -\frac{1}{2} \end{pmatrix} = \begin{pmatrix} \frac{3}{2} \\ -\frac{3}{2} \end{pmatrix}\)

<|ref|>equation<|/ref|><|det|>[[210, 630, 800, 664]]<|/det|>
\(\left|\overrightarrow{AB}\right| = \sqrt{2^2 + (-3)^2 + 2^2} = \sqrt{17} \approx 4,12\)

<|ref|>equation<|/ref|><|det|>[[210, 668, 650, 703]]<|/det|>
\(\overrightarrow{AC} = \overrightarrow{C-A} = \begin{pmatrix} -\frac{1}{2} \\ -\frac{1}{2} \end{pmatrix} - \begin{pmatrix}\frac{3}{2} \\ -\frac{3}{2} \end{pmatrix} = \begin{pmatrix} -\frac{2}{3} \\ -\frac{2}{3} \end{pmatrix}\)

<|ref|>equation<|/ref|><|det|>[[210, 707, 835, 741]]<|/det|>
\(\left|\overrightarrow{AC}\right| = \sqrt{(-2)^2 + (-3)^2 + 4^2} = \sqrt{29} \approx 5,39\)

<|ref|>equation<|/ref|><|det|>[[210, 744, 640, 780]]<|/det|>
\(\overrightarrow{BC} = \overrightarrow{C-B} = \begin{pmatrix} -\frac{1}{2} \\ -\frac{1}{3} \end{pmatrix} - \begin{pmatrix} \frac{3}{2} \\ -\frac{1}{2}  \end{pmatrix} = \begin{pmatrix} -\frac{9}{2} \\ -\frac{9}{2} \end{pmatrix}\)

<|ref|>equation<|/ref|><|det|>[[210, 784, 763, 820]]<|/det|>
\(\left|\overrightarrow{BC}\right| = \sqrt{(-4)^2 + 0^2 + 2^2} = \sqrt{20} \approx 4,47\)

<|ref|>equation<|/ref|><|det|>[[210, 840, 888, 880]]<|/det|>
\(\alpha = \cos^{-1}\left(\frac{\langle\overrightarrow{AB}, \overrightarrow{AC}\rangle}{\|\overrightarrow{AB}\| \|\overrightarrow{AC}\|}\right) = \left(\frac{13}{\sqrt{17} \cdot \sqrt{29}}\right) \approx 54,16^\circ\)

<|ref|>equation<|/ref|><|det|>[[210, 875, 888, 916]]<|/det|>
\(\beta = \cos^{-1}\left(\frac{\langle\overrightarrow{BA}, \overrightarrow{BC}\rangle}{\|\overrightarrow{BA}\| \|\overrightarrow{BC}\|}\right) = \left(\frac{4}{\sqrt{17} \cdot \sqrt{20}}\right) \approx 77,47^\circ\)

<|ref|>equation<|/ref|><|det|>[[210, 920, 580, 958]]<|/det|>
\(\gamma = 180^\circ - \alpha - \beta = 48,37^\circ\)

<|ref|>equation<|/ref|><|det|>[[250, 958, 500, 998]]<|/det|>
\[ = \cos^{-1}\left(\frac{\langle\overrightarrow{AC}, \overrightarrow{BC}\rangle}{\|\overrightarrow{AC}\| \|\overrightarrow{BC}\|}\right) \]