d) Es gilt

$$
\underline{\underline{f^{\prime}(x)}}=2 \cdot 16 \cdot x^{16-1}-7 \cdot 2 \cdot x^{2-1}+3 \cdot 10 \cdot x^{10-1}=\underline{\underline{32 x^{15}-14 x+30 x^{9}}}
$$

e) Es gilt

$$
\underline{\underline{f^{\prime}(x)}}=2 \cdot x^{2-1}+1 \cdot y+0=\underline{\underline{2 x+y}}
$$

f) Wir betrachten die Funktion

$$
f(t)=\frac{1}{t}+t^{\frac{1}{2}} s^{-\frac{1}{2}}-\frac{1}{s}=t^{-1}+t^{\frac{1}{2}} s^{-\frac{1}{2}}-\frac{1}{s}
$$

Es gilt

$$
\underline{\underline{f(t)}}=(-1) \cdot t^{-1-1}+\frac{1}{2} \cdot t^{\frac{1}{2}-1} \cdot s^{-\frac{1}{2}}-0=\underline{\underline{-t^{-2}+\frac{1}{2} \cdot t^{-\frac{1}{2}} s^{-\frac{1}{2}}}}
$$

g) Wir betrachten die Funktion

$$
f(s)=\frac{1}{t}+t^{\frac{1}{2}} s^{-\frac{1}{2}}-s^{-1}
$$

Es gilt

$$
\underline{\underline{f^{\prime}(s)}}=0+t^{\frac{1}{2}} \cdot\left(-\frac{1}{2}\right) \cdot s^{-\frac{1}{2}-1}-(-1) \cdot s^{-1-1}=\underline{\underline{-\frac{1}{2} \cdot t^{\frac{1}{2}} s^{-\frac{3}{2}}+s^{-2}}}
$$

h) Wir betrachten die Funktion

$$
f(x)=2 \cdot(x-1)^{2}=2 \cdot\left(x^{2}-2 x+1\right)
$$

Es gilt

$$
\underline{\underline{f^{\prime}(x)}}=2 \cdot\left(2 \cdot x^{2-1}-2+0\right)=2 \cdot(2 x-2)=\underline{\underline{4 x-4}}
$$

i) Wir betrachten die Funktion

$$
f(y)=(x-y)^{3}=x^{3}-3 x^{2} y+3 x y^{2}-y^{3}
$$

Es gilt

$$
\begin{aligned}
\underline{\underline{f^{\prime}(y)}} & =0-3 x^{2} \cdot 1+3 x \cdot 2 \cdot y^{2-1}-3 \cdot y^{3-1}=-3 x^{2}+6 x y-3 y^{2}=-3 \cdot\left(x^{2}-2 x y+y^{2}\right) \\
& =\underline{\underline{-3 \cdot(x-y)^{2}}}
\end{aligned}
$$