wobei $c \in \mathbb{R}$ beliebig gewählt werden kann.
c) Wir erhalten

$$
f(x)=2 x \Rightarrow\left\{\begin{array}{l}
f^{\prime}(x)=2 \\
F(x)=x^{2}+c
\end{array}\right.
$$

wobei $c \in \mathbb{R}$ beliebig gewählt werden kann.
d) Wir erhalten

$$
f(x)=x \Rightarrow\left\{\begin{array}{l}
f^{\prime}(x)=1 \\
F(x)=\frac{1}{2} x^{2}+c
\end{array}\right.
$$

wobei $c \in \mathbb{R}$ beliebig gewählt werden kann.
e) Wir erhalten

$$
f(x)=3 x \Rightarrow\left\{\begin{array}{l}
f^{\prime}(x)=3 \\
F(x)=\frac{3}{2} x^{2}+c
\end{array}\right.
$$

wobei $c \in \mathbb{R}$ beliebig gewählt werden kann.
f) Wir erhalten

$$
f(x)=x^{2} \Rightarrow\left\{\begin{array}{l}
f^{\prime}(x)=2 x^{2-1}=2 x \\
F(x)=\frac{1}{2+1} x^{2+1}+c=\frac{1}{3} x^{3}+c
\end{array}\right.
$$

wobei $c \in \mathbb{R}$ beliebig gewählt werden kann.
g) Für die Funktion
$f(x)=3 x^{2}+2$
erhalten wir
$\underline{\underline{f^{\prime}(x)}}=3 \cdot 2 \cdot x^{2-1}+0=\underline{\underline{6 x}}$
$\underline{\underline{F(x)}}=3 \cdot \frac{1}{2+1} x^{2+1}+2 x+c=\frac{3}{3} x^{3}+2 x+c=\underline{\underline{x^{3}+2 x+c}}$
wobei $c \in \mathbb{R}$ beliebig gewählt werden kann.
h) Für die Funktion
$f(x)=6 x^{3}-4 x+1$
erhalten wir
$\underline{\underline{f^{\prime}(x)}}=6 x^{3}-4 x+1=6 \cdot 3 \cdot x^{3-1}-4+0=\underline{\underline{18 x^{2}-4}}$