erhalten wir

$$
\begin{aligned}
& \underline{\underline{F(x)}}=\frac{1}{2} \cdot x^{\frac{1}{2}-1}=\frac{1}{2} x^{-\frac{1}{2}}=\frac{1}{2} \cdot \frac{1}{x^{\frac{1}{2}}}=\underline{\underline{2 \sqrt{x}}} \\
& \underline{\underline{F(x)}}=\frac{1}{\frac{1}{2}+1} x^{\frac{1}{2}+1}+c=\frac{1}{\frac{3}{2}} x^{\frac{3}{2}}+c=\underline{\frac{2}{3} \sqrt{x^{3}}+c}
\end{aligned}
$$

wobei $c \in \mathbb{R}$ beliebig gewählt werden kann.
I) Für die Funktion

$$
f(x)=\sqrt{\frac{1}{x}}-1=\sqrt{x^{-1}}-1=\left(x^{-1}\right)^{\frac{1}{2}}-1=x^{-1 \cdot \frac{1}{2}}-1=x^{-\frac{1}{2}}-1
$$

erhalten wir

$$
\begin{aligned}
& \underline{\underline{F(x)}}=-\frac{1}{2} \cdot x^{-\frac{1}{2}-1}-0=-\frac{1}{2} x^{-\frac{3}{2}}=-\frac{1}{2} \cdot \frac{1}{x^{\frac{3}{2}}}=-\underline{\underline{1} \\
& \underline{\underline{F(x)}}=\frac{1}{-\frac{1}{2}+1} x^{-\frac{1}{2}+1}-x+c=\frac{1}{\frac{1}{2}} x^{\frac{1}{2}}-x+c=\underline{\underline{2 \sqrt{x}-x+c}}
\end{aligned}
$$

wobei $c \in \mathbb{R}$ beliebig gewählt werden kann.