<|ref|>text<|/ref|><|det|>[[122, 86, 395, 105]]<|/det|>
a) Wir betrachten das LGLS 

<|ref|>equation<|/ref|><|det|>[[153, 115, 315, 160]]<|/det|>
\[ \begin{cases} 2x - 3y = 6 \\ 5x + 7y = -8, \end{cases} \]

<|ref|>text<|/ref|><|det|>[[153, 172, 545, 190]]<|/det|>
welches äquivalent ist zum GAUSS-Schema 

<|ref|>table<|/ref|><|det|>[[152, 201, 288, 253]]<|/det|>
<table><tr><td>2</td><td>-3</td><td>6</td></tr><tr><td>5</td><td>7</td><td>-8</td></tr></table>

<|ref|>text<|/ref|><|det|>[[153, 271, 444, 291]]<|/det|>
Offensichtlich gilt \(n_V = n_G = 2\). 

<|ref|>text<|/ref|><|det|>[[122, 300, 397, 318]]<|/det|>
b) Wir betrachten das LGLS 

<|ref|>equation<|/ref|><|det|>[[153, 330, 303, 400]]<|/det|>
\[ \begin{cases} x + y = 1 \\ x - y = -2 \\ 2x - y = 1, \end{cases} \]

<|ref|>text<|/ref|><|det|>[[122, 410, 536, 429]]<|/det|>
welches äquivalent ist zum GAUSS-Schema 

<|ref|>table<|/ref|><|det|>[1.5cm] 
<table><tr><td>1</td><td>1</td><td>1</td></tr><tr><td>1</td><td>-1</td><td>-2</td></tr><tr><td>2</td><td>-1</td><td>1</td></tr></table>

<|ref|>text<|/ref|><|det|>[[122, 543, 491, 563]]<|/det|>
Offensichtlich gilt \(n_V = 2\) und \(n_G = 3\). 

<|ref|>text<|/ref|><|det|>[[122, 571, 383, 589]]<|/det|>
c) Wir betrachten das LGLS 

<|ref|>equation<|/ref|><|det|>[[153, 600, 550, 647]]<|/det|>
\[ \begin{cases} 1 + x = y - 1 \\ 2y - x + 3 = 0 \end{cases} \Leftrightarrow \begin{cases} x - y = -2 \\ -x + 2y = -3, \end{cases} \]

<|ref|>text<|/ref|><|det|>[[153, 658, 525, 675]]<|/det|>
welches äquivalent ist zum GAUSS-Schema 

<|ref|>table<|/ref|><|det|>[-1.5cm] 
<table><tr><td>1</td><td>-1</td><td>-2</td></tr><tr><td>-1</td><td>2</td><td>-3</td></tr></table>

<|ref|>text<|/ref|><|det|>[[153, 755, 428, 774]]<|/det|>
Offensichtlich gilt \(n_V = n_G = 2\).