<|ref|>equation<|/ref|><|det|>[[113, 80, 707, 180]]<|/det|>
\[
\begin{align*}
\text{g)} & \left\langle \begin{pmatrix} \cos \varphi \\ \sin \varphi \end{pmatrix}, \begin{pmatrix} \cos \varphi \\ -\sin \varphi \end{pmatrix} \right\rangle \\
\text{i)} & \left\langle \begin{pmatrix} 2^x \\ 3^x \end{pmatrix}, \begin{pmatrix} 2^{-x} \\ 3^x \end{pmatrix} \right\rangle
\end{align*}
\]

<|ref|>text<|/ref|><|det|>[[115, 193, 144, 207]]<|/det|>
a) 

<|ref|>equation<|/ref|><|det|>[[119, 211, 519, 255]]<|/det|>
\[
\left\langle \begin{bmatrix} 1 \\ 2 \end{bmatrix}, \begin{bmatrix} 3 \\ 4 \end{bmatrix} \right\rangle = 1 \cdot 3 + 2 \cdot 4 = 3 + 8 = \underline{11}
\]

<|ref|>text<|/ref|><|det|>[[115, 262, 144, 276]]<|/det|>
b) 

<|ref|>equation<|/ref|><|det|>[[119, 277, 595, 320]]<|/det|>
\[
\left\langle \begin{bmatrix} 2 \\ 4 \end{bmatrix}, \begin{bmatrix} -6 \\ 3 \end{bmatrix} \right\rangle = 2 \cdot (-6) + 4 \cdot 3 = -12 + 12 = \underline{0}
\]

<|ref|>text<|/ref|><|det|>[[115, 327, 144, 341]]<|/det|>
c) 

<|ref|>equation<|/ref|><|det|>[[119, 341, 650, 405]]<|/det|>
\[
\left\langle \begin{bmatrix} 1 \\ 2 \\ 3 \end{bmatrix}, \begin{bmatrix} 4 \\ 5 \\ 6 \end{bmatrix} \right\rangle = 1 \cdot 4 + 2 \cdot 5 + 3 \cdot 6 = 4 + 10 + 18 = \underline{32}
\]

<|ref|>text<|/ref|><|det|>[[115, 412, 144, 427]]<|/det|>
d) 

<|ref|>equation<|/ref|><|det|>[[119, 430, 875, 503]]<|/det|>
\[
\left\langle \begin{bmatrix} -3 \\ 0 \\ -\sqrt{2} \end{bmatrix}, \begin{bmatrix} -1 \\ 1 \\ \sqrt{8} \end{bmatrix} \right\rangle = (-3) \cdot (-1) + 0 \cdot 1 - \sqrt{2} \cdot \sqrt{8} = 3 + 0 - \sqrt{2} \cdot 8 = 3 - \sqrt{16}
\]

<|ref|>equation<|/ref|><|det|>[[338, 515, 472, 536]]<|/det|>
\[
= 3 - 4 = \underline{-1}.
\]

<|ref|>text<|/ref|><|det|>[[115, 536, 144, 550]]<|/det|>
e) 

<|ref|>equation<|/ref|><|det|>[[119, 553, 841, 640]]<|/det|>
\[
\left\langle \begin{bmatrix} 1 \\ -1 \\ -1 \end{bmatrix}, \begin{bmatrix} 2 \\ -3 \\ -3 \end{bmatrix} \right\rangle = 1 \cdot 2 + (-1) \cdot (-3) + 1 \cdot (-3) + (-1) \cdot 2 = 2 + 3 - 3 - 2
\]

<|ref|>equation<|/ref|><|det|>[[323, 658, 368, 680]]<|/det|>
\[
= \underline{0}.
\]

<|ref|>text<|/ref|><|det|>[[115, 680, 144, 695]]<|/det|>
f) 

<|ref|>equation<|/ref|><|det|>[[119, 695, 780, 782]]<|/det|>
\[
\left\langle \begin{bmatrix} 0.2 \\ -\sqrt{3} \\ 0 \\ -\frac{1}{2} \end{bmatrix}, \begin{bmatrix} -3 \\ \sqrt{3} \\ -\sqrt{7} \\ -3 \end{bmatrix} \right\rangle = 0.2 \cdot (-3) - \sqrt{3} \cdot \sqrt{3} + 0 \cdot \left(-\sqrt{7}\right) - \frac{1}{2} \cdot (-3)
\]

<|ref|>equation<|/ref|><|det|>[[350, 799, 768, 835]]<|/det|>
\[
= -0.6 - 3 + 0 + \frac{3}{2} = -0.6 - 3 + 1.5 = \underline{-2.1}.
\]