<|ref|>text<|/ref|><|det|>[[114, 83, 145, 100]]<|/det|>
b) 

<|ref|>image<|/ref|><|det|>[[114, 100, 595, 352]]<|/det|>
 

<|ref|>text<|/ref|><|det|>[[114, 355, 264, 372]]<|/det|>
Seitenvektoren: 

<|ref|>equation<|/ref|><|det|>[[117, 372, 620, 510]]<|/det|>
\[
\begin{align*}
\mathbf{a} := \mathbf{C} - \mathbf{B} &= \begin{bmatrix} 1 \\ 1 \end{bmatrix} - \begin{bmatrix} 4 \\ 1 \end{bmatrix} = \begin{bmatrix} 1 - 4 \\ 1 - 1 \end{bmatrix} = \begin{bmatrix} -3 \\ 0 \end{bmatrix} \\
\mathbf{b} := \mathbf{A} - \mathbf{C} &= \begin{bmatrix} -1 \\ -2 \end{bmatrix} - \begin{bmatrix} 1 \\ 1 \end{bmatrix} = \begin{bmatrix} -1 - 1 \\ -2 - 1 \end{bmatrix} = \begin{bmatrix} -2 \\ -3 \end{bmatrix} \\
\mathbf{c} := \mathbf{B} - \mathbf{A} &= \begin{bmatrix} 4 \\ 1 \end{bmatrix} - \begin{bmatrix} -1 \\ -2 \end{bmatrix} = \begin{bmatrix} 4 - (-1) \\ 1 - (-2) \end{bmatrix} = \begin{bmatrix} 5 \\ 3 \end{bmatrix}
\end{align*}
\]

<|ref|>text<|/ref|><|det|>[[114, 508, 245, 526]]<|/det|>
Seitenl√§ngen: 

<|ref|>equation<|/ref|><|det|>[[117, 525, 536, 550]]<|/det|>
\[
\underline{a} = |\mathbf{a}| = \sqrt{\langle \mathbf{a}, \mathbf{a} \rangle} = \sqrt{(-3)^2 + 0^2} = \sqrt{9} = \frac{3}{2}
\]

<|ref|>equation<|/ref|><|det|>[[117, 560, 544, 587]]<|/det|>
\[
\underline{b} = |\mathbf{b}| = \sqrt{\langle \mathbf{b}, \mathbf{b} \rangle} = \sqrt{(-2)^2 + (-3)^2} = \sqrt{13}
\]

<|ref|>equation<|/ref|><|det|>[[117, 597, 575, 624]]<|/det|>
\[
\underline{c} = |\mathbf{c}| = \sqrt{\langle \mathbf{c}, \mathbf{c} \rangle} = \sqrt{5^2 + 3^2} = \sqrt{34} = \frac{\sqrt{2}}{\sqrt{17}}.
\]

<|ref|>text<|/ref|><|det|>[[114, 623, 234, 640]]<|/det|>
Innenwinkel: 

<|ref|>equation<|/ref|><|det|>[[117, 637, 740, 912]]<|/det|>
\[
\begin{align*}
\underline{\alpha} &= \angle(-\mathbf{b}, \mathbf{c}) = \arccos\left(\frac{-\langle\mathbf{b}, \mathbf{c}\rangle}{|\mathbf{b}| \cdot |\mathbf{c}|}\right) = \arccos\left(\frac{-(-2) \cdot 5 - (-3) \cdot 3}{\sqrt{13} \sqrt{2} \sqrt{17}}\right) \\
&= \arccos\left(\frac{19}{\sqrt{13} \sqrt{2} \sqrt{17}}\right) \approx 0.442'37 \approx 0.141\pi
\end{align*}
\]

<|ref|>equation<|/ref|><|det|>[[117, 737, 777, 912]]<|/det|>
\[
\begin{align*}
\underline{\beta} &= \angle(-\mathbf{c}, \mathbf{a}) = \arccos\left(\frac{-\langle\mathbf{c}, \mathbf{a}\rangle}{|\mathbf{c}| \cdot |\mathbf{a}|}\right) = \arccos\left(\frac{-5 \cdot (-3) - 3 \cdot 0}{\sqrt{2} \sqrt{17} \cdot 3}\right) \\
&= \arccos\left(\frac{15}{3 \sqrt{2} \sqrt{17}}\right) = \arccos\left(\frac{5}{\sqrt{2} \sqrt{17}}\right) \approx 0.540'42 \approx 0.172\pi
\end{align*}
\]

<|ref|>equation<|/ref|><|det|>[[117, 830, 777, 912]]<|/det|>
\[
\underline{\gamma} = \angle(-\mathbf{a}, \mathbf{b}) = \arccos\left(\frac{-\langle\mathbf{a}, \mathbf{b}\rangle}{|\mathbf{a}| \cdot |\mathbf{b}|}\right) = \arccos\left(\frac{-(-3) \cdot (-2) - 0 \cdot (-3)}{3 \sqrt{13}}\right) \\
&= \arccos\left(\frac{-6}{3 \sqrt{13}}\right) = \arccos\left(\frac{-2}{\sqrt{13}}\right) \approx 2.158'8 \approx 0.687\pi.
\]