<|ref|>text<|/ref|><|det|>[[30, 17, 700, 45]]<|/det|>
Bayes - Formel - ergibt sich aus Multiplikationssatz : 

<|ref|>equation<|/ref|><|det|>[[58, 50, 320, 85]]<|/det|>
\[P(A|B) = \frac{P(B|A)}{P(B)} \cdot P(A)\]

<|ref|>text<|/ref|><|det|>[[30, 97, 565, 123]]<|/det|>
Satz von Bayes : \(A_1, \ldots, A_n\) seien disjunkt 

<|ref|>equation<|/ref|><|det|>[[58, 131, 470, 214]]<|/det|>
\[P(A_j|B) = \frac{P(B|A_j)}{\sum_{i=1}^{n} P(B|A_i) \cdot P(A_i)} \cdot P(A_j) = P(B)\]

<|ref|>text<|/ref|><|det|>[[30, 246, 600, 272]]<|/det|>
Totale wahrscheinlichkeit : \(A_i\) seien disjunkt 

<|ref|>equation<|/ref|><|det|>[[386, 285, 692, 309]]<|/det|>
\[A_1 \cup A_2 \cup \ldots \cup A_n = \Omega\]

<|ref|>equation<|/ref|><|det|>[[58, 319, 365, 353]]<|/det|>
\[P(B) = \sum_{i} P(A_i) \cdot P(B|A_i)\]