<|ref|>text<|/ref|><|det|>[[125, 87, 230, 105]]<|/det|>
Es gilt also 

<|ref|>equation<|/ref|><|det|>[[296, 116, 812, 167]]<|/det|>
\[ 
\begin{aligned}
F(x) &= -\sin(x) \cos(x) + x + b - F(x) \\
2 \cdot F(x) &= -\sin(x) \cos(x) + x + b
\end{aligned}
\quad \begin{aligned}
| + F(x) & | : 2.
\end{aligned} 
\]

<|ref|>text<|/ref|><|det|>[[125, 175, 304, 193]]<|/det|>
Daraus erhalten wir 

<|ref|>equation<|/ref|><|det|>[[125, 200, 615, 238]]<|/det|>
\[ \frac{F(x)}{2} = \frac{-\sin(x) \cos(x) + x + b}{2} = \frac{x - \sin(x) \cos(x)}{2} + c. \]

<|ref|>text<|/ref|><|det|>[[115, 243, 144, 261]]<|/det|>
h) 

<|ref|>equation<|/ref|><|det|>[[115, 262, 512, 303]]<|/det|>
\[ F(x) = \int \cos^2(x) \, dx = \int \cos(x) \cdot \cos(x) \, dx \]

<|ref|>equation<|/ref|><|det|>[[161, 323, 856, 432]]<|/det|>
\[ 
\begin{aligned}
& = \cos(x) \cdot \sin(x) - \int (- \sin(x)) \cdot \sin(x) \, dx = \cos(x) \sin(x) + \int \sin^2(x) \, dx \\
& = \cos(x) \sin(x) + \int (1 - \cos^2(x)) \, dx = \cos(x) \sin(x) + \int 1 \, dx - \int \cos^2(x) \, dx \\
& = \cos(x) \sin(x) + x + b - F(x).
\end{aligned}
\]

<|ref|>text<|/ref|><|det|>[[120, 435, 230, 453]]<|/det|>
Es gilt also 

<|ref|>equation<|/ref|><|det|>[[315, 466, 820, 485]]<|/det|>
\[ | + F(x) | + F(x) \]

<|ref|>equation<|/ref|><|det|>[[301, 495, 785, 515]]<|/det|>
\[ 2 \cdot F(x) = \cos(x) \sin(x) + x + b \quad | : 2. \]

<|ref|>text<|/ref|><|det|>[[120, 528, 303, 546]]<|/det|>
Daraus erhalten wir 

<|ref|>equation<|/ref|><|det|>[[120, 555, 600, 595]]<|/det|>
\[ \frac{F(x)}{2} = \frac{\cos(x) \sin(x) + x + b}{2} = \frac{x + \cos(x) \sin(x)}{2} + c. \]

<|ref|>text<|/ref|><|det|>[[115, 597, 140, 615]]<|/det|>
i) 

<|ref|>equation<|/ref|><|det|>[[125, 625, 520, 666]]<|/det|>
\[ F(x) = \int \sinh^2(x) \, dx = \int \sinh(x) \cdot \sinh(x) \, dx \]

<|ref|>equation<|/ref|><|det|>[[167, 686, 880, 789]]<|/det|>
\[ 
\begin{aligned}
& = \sinh(x) \cdot \cosh(x) - \int \cosh(x) \cdot \cosh(x) \, dx = \sinh(x) \cosh(x) - \int \cosh^2(x) \, dx \\
& = \sinh(x) \cosh(x) - \int (1 + \sinh^2(x)) \, dx = \sinh(x) \cosh(x) - \int 1 \, dx - \int \sinh^2(x) \, dx \\
& = \sinh(x) \cosh(x)
\end{aligned}
\]