<|ref|>text<|/ref|><|det|>[[114, 84, 142, 101]]<|/det|>
b) 

<|ref|>equation<|/ref|><|det|>[[125, 103, 730, 184]]<|/det|>
\[
\begin{align*}
F(x) &= \int x^2 \cdot e^x \, dx = x^2 e^x - \int 2x \cdot e^x \, dx = x^2 e^x - 2(x-1)e^x + c \\
&= (x^2 - 2x + 2)e^x + c.
\end{align*}
\]

<|ref|>text<|/ref|><|det|>[[114, 187, 142, 204]]<|/det|>
c) 

<|ref|>equation<|/ref|><|det|>[[125, 204, 856, 295]]<|/det|>
\[
\begin{align*}
F(x) &= \int x \cdot \sin(x) \, dx = x \cdot \left(-\cos(x)\right) - \int 1 \cdot \left(-\cos(x)\right) \, dx \\
&= -x \cos(x) + \int \cos(x) \, dx = -x \cos(x) + \sin(x) + c = \sin(x) - x \cos(x) + c.
\end{align*}
\]

<|ref|>text<|/ref|><|det|>[[114, 295, 142, 312]]<|/det|>
d) 

<|ref|>equation<|/ref|><|det|>[[125, 315, 808, 360]]<|/det|>
\[
F(x) = \int x \cdot \cos(x) \, dx = x \cdot \sin(x) - \int 1 \cdot \sin(x) \, dx = \frac{x \sin(x) + \cos(x) + c}{2}
\]

<|ref|>text<|/ref|><|det|>[[114, 361, 142, 378]]<|/det|>
e) 

<|ref|>equation<|/ref|><|det|>[[125, 378, 810, 500]]<|/det|>
\[
\begin{align*}
F(x) &= \int x^2 \cdot \sin(x) \, dx = x^2 \cdot \left(-\cos(x)\right) - \int 2x \cdot \left(-\cos(x)\right) \, dx \\
&= -x^2 \cos(x) + 2 \int x \cos(x) \, dx = -x^2 \cos(x) + 2x \sin(x) + 2 \cos(x) + c \\
&= 2x \sin(x) + (2 - x^2) \cos(x) + c.
\end{align*}
\]

<|ref|>text<|/ref|><|det|>[[114, 501, 142, 518]]<|/det|>
f) 

<|ref|>equation<|/ref|><|det|>[[125, 518, 880, 600]]<|/det|>
\[
\begin{align*}
F(x) &= \int x^2 \cdot
\cos(x) \, dx = x^2 \cdot \sin(x) - \int 2x \cdot \sin(x) \, dx = x^2 \sin(x) - 2 \int x \sin(x) \, dx \\
&= x^2 \sin(x) - 2 \sin(x) + 2x \cos(x) + c = \left(x^2 - 2\right) \sin(x) + 2x \cos(x) + c.
\end{align*}
\]

<|ref|>text<|/ref|><|det|>[[114, 602, 142, 619]]<|/det|>
g) 

<|ref|>equation<|/ref|><|det|>[[125, 618, 880, 784]]<|/det|>
\[
\begin{align*}
F(x) &= \int \sin^2(x) \, dx = \int \sin(x) \cdot \sin(x) \, dx \\
&= \sin(x) \cdot \left(-\cos(x)\right) - \int \cos(x) \cdot \left(-\cos(x)\right) \, dx = -\sin(x) \cos(x) + \int \cos^2(x) \, dx \\
&= -\sin(x) \cos(x) + \int \left(1 - \sin^2(x)\right) \, dx = -\sin(x) \cos(x) + \int 1 \, dx - \int \sin^2(x) \, dx \\
&= -\sin(x) \cos(x) + x + b - F(x).
\end{align*}
\]