<|ref|>text<|/ref|><|det|>[[115, 84, 140, 100]]<|/det|>
a) 

<|ref|>equation<|/ref|><|det|>[[120, 103, 644, 140]]<|/det|>
\[
\frac{F(x)}{=} \int (2x+7)^3 \, \mathrm{d}x = \frac{1}{2} \cdot \frac{1}{4} \cdot (2x+7)^4 + c = \frac{1}{8} (2x+7)^4 + c.
\]

<|ref|>text<|/ref|><|det|>[[115, 140, 140, 156]]<|/det|>
b) 

<|ref|>equation<|/ref|><|det|>[[120, 159, 725, 260]]<|/det|>
\[
\begin{align*}
\frac{F(x)}{=} \int (4-2x)^7 \, \mathrm{d}x &= \frac{1}{-2} \cdot \frac{1}{8} \cdot (4-2x)^8 + c = -\frac{1}{16} (4-2x)^8 + c \\
&= -\frac{1}{16} (2 \cdot (2-x))^8 + c = -\frac{1}{24} \cdot 2^8 \cdot (2-x)^8 + c = -2^4 \cdot (2-x)^8 + c \\
&= -16 (2-x)^8 + c.
\end{align*}
\]

<|ref|>text<|/ref|><|det|>[[115, 266, 140, 282]]<|/det|>
c) 

<|ref|>equation<|/ref|><|det|>[[120, 286, 651, 325]]<|/det|>
\[
\frac{F(x)}{=} \int 9 \cdot 2^{3x-5} \, \mathrm{d}x = 9 \cdot \frac{1}{3 \ln(2)} \cdot 2^{3x-5} + c = \frac{3}{\ln(2)} \cdot 2^{3x-5} + c.
\]

<|ref|>text<|/ref|><|det|>[[115, 330, 140, 346]]<|/det|>
d) 

<|ref|>equation<|/ref|><|det|>[[120, 350, 640, 390]]<|/det|>
\[
\frac{F(x)}{=} \int \frac{1}{5} \cdot 2^{\frac{x-10}{15}} \, \mathrm{d}x = \frac{1}{5} \cdot \frac{15}{\ln(2)} \cdot 2^{\frac{x-10}{15}} + c = \frac{3}{\ln(2)} \cdot 2^{\frac{x-10}{15}} + c.
\]

<|ref|>text<|/ref|><|det|>[[115, 395, 140, 410]]<|/det|>
e) 

<|ref|>equation<|/ref|><|det|>[[120, 415, 656, 494]]<|/det|>
\[
\begin{align*}
\frac{F(x)}{=} \int \frac{1}{\sqrt{4x-3}} \, \mathrm{d}x &= \int (4x-3)^{-\frac{1}{2}} \, \mathrm{d}x = \frac{1}{4} \cdot \frac{1}{\frac{1}{2}} \cdot (4x-3)^{\frac{1}{2}} + c \\
&= \frac{1}{2} \sqrt{4x-3} + c.
\end{align*}
\]

<|ref|>text<|/ref|><|det|>[[115, 496, 135, 512]]<|/det|>
f) 

<|ref|>equation<|/ref|><|det|>[[120, 515, 636, 592]]<|/det|>
\[
\begin{align*}
F(x) &= \int \sqrt{6-x} \, \mathrm{d}x = \int (6-x)^{\frac{1}{2}} \, \mathrm{d}x = \frac{1}{-1} \cdot \frac{1}{\frac{3}{2}} \cdot (6-x)^{\frac{3}{2}} + c \\
&= -\frac{2}{3} \sqrt{(6-x)^3} + c.
\end{align*}
\]

<|ref|>text<|/ref|><|det|>[[115, 595, 140, 611]]<|/det|>
g) 

<|ref|>equation<|/ref|><|det|>[[120, 616, 653, 654]]<|/det|>
\[
\frac{F(x)}{=} \int (5x-3)^2 \, \mathrm{d}x = \frac{1}{5} \cdot \frac{1}{3} \cdot (5x-3)^3 + c = \frac{1}{15} (5x-3)^3 + c.
\]

<|ref|>text<|/ref|><|det|>[[115, 658, 140, 674]]<|/det|>
h) 

<|ref|>equation<|/ref|><|det|>[[120, 678, 768, 717]]<|/det|>
\[
\frac{F(x)}{=} \int (3-0.25x)^7 \, \mathrm{d}x = \frac{1}{-0.25} \cdot \frac{1}{8} \cdot (3-0.25x)^8 + c = -\frac{1}{2} (3-0.25x)^8 + c.
\]

<|ref|>text<|/ref|><|det|>[[115, 720, 135, 736]]<|/det|>
i) 

<|ref|>equation<|/ref|><|det|>[[120, 740, 712, 780]]<|/det|>
\[
\frac{F(x)}{=} \int 12 \cdot 7^{5-3x} \, \mathrm{d}x = 12 \cdot \frac{1}{-3} \cdot \frac{1}{\ln(7)} \cdot 7^{5-3x} + c = -\frac{4}{\ln(7)} \cdot 7^{5-3x} + c.
\]

<|ref|>text<|/ref|><|det|>[[115, 784, 135, 800]]<|/det|>
j) 

<|ref|>equation<|/ref|><|det|>[[120, 804, 640, 843]]<|/det|>
\[
\frac{F(x)}{=} \int \frac{1}{6} \cdot 2^{\frac{x-11}{18}} \, \mathrm{d}x = \frac{1}{6} \cdot \frac{18}{\ln(2)} \cdot 2^{\frac{x-11}{18}} + c = \frac{3}{\ln(2)} \cdot 2^{\frac{11}{18}} + c.
\]