<|ref|>text<|/ref|><|det|>[[115, 83, 144, 100]]<|/det|>
b) 

<|ref|>equation<|/ref|><|det|>[[117, 99, 820, 184]]<|/det|>
\[
\begin{align*}
\underline{I} &= \int_0^2 \int_0^1 x^2 \, \mathrm{d}x \, \mathrm{d}y = \int_0^1 x^2 \, \mathrm{d}x \cdot \int_0^2 1 \, \mathrm{d}y = \frac{1}{3} \cdot \left[ x^3 \right]_0^1 \cdot \left[ y \right]_0^2 = \frac{1}{3} \cdot (1^3 - 0) \cdot (2 - 0) \\
&= \frac{1}{3} \cdot 1 \cdot 2 = \frac{2}{3}.
\end{align*}
\]

<|ref|>text<|/ref|><|det|>[[115, 214, 144, 231]]<|/det|>
c) 

<|ref|>equation<|/ref|><|det|>[[117, 230, 825, 345]]<|/det|>
\[
\begin{align*}
\underline{I} &= \int_0^{\ln(3)} \int_0^{\ln(2)} \mathrm{e}^{2x+y} \, \mathrm{d}x \, \mathrm{d}y = \int_0^{\ln(3)} \int_0^{\ln(2)} \left( \mathrm{e}^{2x} \cdot \mathrm{e}^y \right) \, \mathrm{d}x \, \mathrm{d}y = \int_0^{\ln(2)} \mathrm{e}^{2x} \, \mathrm{d}x \cdot \int_0^{\ln(3)} \mathrm{e}^y \, \mathrm{d}y \\
&= \frac{1}{2} \cdot \left[ \mathrm{e}^{2x} \right]_0^{\ln(2)} \cdot \left[ \mathrm{e}^y \right]_0^{\ln(3)} = \frac{1}{2} \cdot (\mathrm{e}^{2\ln(2)} - \mathrm{e}^0) \cdot (\mathrm{e}^{\ln(3)} - \mathrm{e}^0) = \frac{1}{2} \cdot (2^2 - 1) \cdot (3 - 1) \\
&= \frac{1}{2} \cdot (4 - 1) \cdot 2 = \frac{1}{2} \cdot 3 \cdot 2 = \frac{3}{2}.
\end{align*}
\]

<|ref|>text<|/ref|><|det|>[[115, 346, 144, 363]]<|/det|>
d) 

<|ref|>equation<|/ref|><|det|>[[117, 360, 819, 440]]<|/det|>
\[
\begin{align*}
\underline{I} &= \int_0^1 \int_1^{\mathrm{e}} \frac{x^2}{y} \, \mathrm{d}y \, \mathrm{d}x = \int_0^1 x^2 \, \mathrm{d}x \cdot \int_{1}^{\mathrm{e}} \frac{1}{y} \, \mathrm{d}y = \frac{1}{3} \cdot \left[ x^{3} \right]_0^1 \cdot \ln\left(\frac{\mathrm{e}}{1}\right) = \frac{1}{3} \cdot (1^3 - 0) \ln(\mathrm{e}) \\
&= \frac{1}{3} \cdot 1 \cdot 1 = \frac{1}{3}.
\end{align*}
\]

<|ref|>text<|/ref|><|det|>[[115, 440, 144, 457]]<|/det|>
e) 

<|ref|>equation<|/ref|><|det|>[[117, 455, 803, 536]]<|/det|>
\[
\begin{align*}
\underline{I} &= \int_{-1}^{4} \int_{-1}^{2} (2x + 6x^2y) \, \mathrm{d}x \, \mathrm{d}y = \int_{-1}^{4} \left[ x^2 + 2x^3y \right]_{-1}^{2} \, \mathrm{d}y = \int_{-1}^{4} (4 + 16y - 1 + 2y) \, \mathrm{d}y \\
&= \int_{-1}^{4} (3 + 18y) \, \mathrm{d}y = \left[ 3y + 9y^2 \right]_{-1}^{4} = 12 + 144 - 3 - 9 = \underline{144}.
\end{align*}
\]

<|ref|>text<|/ref|><|det|>[[115, 536, 144, 554]]<|/det|>
f) 

<|ref|>equation<|/ref|><|det|>[[117, 552, 860, 644]]<|/det|>
\[
\begin{align*}
\underline{I} &= \int_{-1}^{2} \int_{-1}^{4} (2x + 6x^2y) \, \mathrm{d}y \, \mathrm{d}x = \int_{-1}^{2} \left[ 2xy + 3x^2y^2 \right]_{-1}^{4} \, \mathrm{d}x = \int_{-1}^{2} (8x + 48x^2 - 2x - 3x^2) \, \mathrm{d}x \\
&= \int_{-1}^{2} (6x + 45x^2) \, \mathrm{d}x = \left[ 3x^2 + 15x^3 \right]_{-1}^{2} = 12 + 120 - 3 + 15 = \underline{144}.
\end{align*}
\]

<|ref|>text<|/ref|><|det|>[[115, 656, 315, 673]]<|/det|>
3. Zweifachintegrale 

<|ref|>text<|/ref|><|det|>[[115, 672, 468, 690]]<|/det|>
Berechnen Sie die folgenden Integrale. 

<|ref|>equation<|/ref|><|det|>[[115, 689, 739, 718]]<|/det|>
a) \(\int_0^2 f_{y^2}^{2y}(4x-y) \, dx \, dy\) b) \(\int_1^2 f_{1-x}^{x^2} x^2 y \, dy \, dx\) c) \(\int_1^2 f_0^x e^x \, dy \, dx\) 

<|ref|>text<|/ref|><|det|>[[115, 735, 144, 752]]<|/det|>
a) 

<|ref|>equation<|/ref|><|det|>[[117, 750, 825, 921]]<|/det|>
\[
\begin{align*}
\underline{I} &= \int_0^2 y^2 \int_0^{2y} (4x-y) \, \mathrm{d}x \, \mathrm{d}y = \int_0^2 \left[ 2x^2 - yx \right]_{y^2}^{2y} \, \mathrm{d}y \\
&= \int_0^2 (2 \cdot 4y^2 - y \cdot 2y - 2 \cdot y^4 + y \cdot y^2) \, \mathrm{d}y = \int_0^2 (6y^2 - 2y^4 + y^3) \, \mathrm{d}y \\
&= \left[ 2y^3 - \frac{2y^5}{5} + \frac{y^4}{4} \right]_0^2 = 2 \cdot 2^3 - \frac{2 \cdot 2^5}{5} + \frac{2^4}{4} - 0 + 0 - 0 = 16 - \frac{64}{5} + 4 = 20 - \frac{64}{5} \\
&= \frac{100}{5} - \frac{64}{5} = \frac{36}{5}.
\end{align*}
\]