<|ref|>equation<|/ref|><|det|>[[120, 85, 642, 145]]<|/det|>
\[A_1 = \left| 0,2 \cdot \int_{0}^{2} (x^3 - 4x) \, dx \right| = \left| 0,2 \left[ \frac{1}{4} x^4 - 2x^2 \right]_{0}^{2} \right| = 0,8\]

<|ref|>equation<|/ref|><|det|>[[120, 148, 600, 203]]<|/det|>
\[A_2 = 0,2 \cdot \int_{\frac{3}{2}}^{3} (x^3 - 4x) \, dx = 0,2 \left[ \frac{1}{4} x^4 - 3x^2 \right]_{\frac{3}{2}}^{3} = 1,25\]

<|ref|>equation<|/ref|><|det|>[[114, 205, 300, 224]]<|/det|>
\[A = 2(A_1 + A_2) = 4,1\]

<|ref|>image<|/ref|><|det|>[[114, 241, 483, 440]]<|/det|>
 

<|ref|>text<|/ref|><|det|>[[114, 440, 144, 458]]<|/det|>
b) 

<|ref|>image<|/ref|><|det|>[[114, 459, 383, 685]]<|/det|>
 

<|ref|>text<|/ref|><|det|>[[114, 690, 808, 710]]<|/det|>
Gleichsetzen der beiden Funktionen, um die Integrationsgrenzen zu erhalten: 

<|ref|>equation<|/ref|><|det|>[[120, 711, 390, 731]]<|/det|>
\[x^2 - 2 = -x^2 + 2x + 2 \quad \Rightarrow\]

<|ref|>equation<|/ref|><|det|>[[120, 736, 525, 757]]<|/det|>
\[2(x^2 - x - 2) = 0 \quad \Rightarrow \quad x_1 = -1; \quad x_2 = 2\]

<|ref|>equation<|/ref|><|det|>[[120, 761, 503, 811]]<|/det|>
\[A = \int_{-1}^{2} \left[ (-x^2 + 2x + 2) - (x^2 - 2) \right] \, dx =\]

<|ref|>equation<|/ref|><|det|>[[140, 817, 400, 867]]<|/det|>
\[= \int_{-1}^{2} (-2x^2 + 2x + 4) \, dx =\]

<|ref|>equation<|/ref|><|det|>[[140, 872, 420, 922]]<|/det|>
\[= \left[ -\frac{2}{3}x^3 + x^2 + 4x \right]_{-1}^{2} = 9\]