e) Wir erhalten

$$
\begin{aligned}
& \underline{\underline{F(x)}}=\int 3^{2+x} \mathrm{~d} x=\int 3^{2} \cdot 3^{x} \mathrm{~d} x=9 \int 3^{x} \mathrm{~d} x=9 \cdot \frac{1}{\ln (3)} \cdot 3^{x}+c=\frac{9}{\ln (3)} \cdot 3^{x}+c \\
& =\underline{\underline{\frac{1}{\ln (3)}} \cdot 3^{2+x}+c .}
\end{aligned}
$$

f) Wir erhalten

$$
\begin{aligned}
& \underline{\underline{F(x)}}=\int \frac{1}{3^{x-2}} \mathrm{~d} x=\int \frac{1}{3^{x} \cdot 3^{-2}} \mathrm{~d} x=\frac{1}{3^{-2}} \int \frac{1}{3^{x}} \mathrm{~d} x=\frac{1}{3^{-2}} \int\left(\frac{1}{3}\right)^{x} \mathrm{~d} x \\
& =\frac{1}{3^{-2}} \cdot \frac{1}{\ln \left(\frac{1}{3}\right)} \cdot\left(\frac{1}{3}\right)^{x}+c=\frac{1}{3^{-2}} \cdot \frac{1}{-\ln (3)} \cdot \frac{1}{3^{x}}+c=\underline{\frac{1}{\ln (3)} \cdot \frac{1}{3^{x-2}}+c .}
\end{aligned}
$$