\# Parameter:
$f=2 * x+1 ;$
Gemäss Ausgabe erhalten wir die Aufleitung
$\underline{F(x)=x^{2}+x+c .}$
b) Wir modifizieren den Code.
\# Parameter:
$f=4 * x-8 ;$
Gemäss Ausgabe erhalten wir die Aufleitung
$\underline{F(x)=2 x^{2}-8 x+c .}$
c) Wir modifizieren den Code.
\# Parameter:
$f=12 * x * * 2+17 ;$
Gemäss Ausgabe erhalten wir die Aufleitung
$\underline{F(x)=4 x^{3}+17 x+c .}$
d) Wir modifizieren den Code.
\# Parameter:
$f=3 * x * * 2-6 * x ;$
Gemäss Ausgabe erhalten wir die Aufleitung
$\underline{F(x)=x^{3}-3 x^{2}+c .}$
e) Wir modifizieren den Code.
\# Parameter:
$f=6 * x * * 2-4 * x+3 ;$
Gemäss Ausgabe erhalten wir die Aufleitung
$\underline{F(x)=2 x^{3}-2 x^{2}+3 x+c .}$
f) Wir modifizieren den Code.
\# Parameter:
$f=8 * x-1+9 * x * * 2 ;$
Gemäss Ausgabe erhalten wir die Aufleitung
$\underline{F(x)=3 x^{3}+4 x^{2}-x+c .}$