<|ref|>equation<|/ref|><|det|>[[120, 78, 650, 375]]<|/det|>
\[
\begin{align*}
\text{det} \left[ \begin{array}{ccc} 1-\lambda & 0 & 0 \\ 2 & 2-\lambda & -1 \\ 0 & -3 & -\lambda \end{array} \right] &= \begin{array}{ccc} 1-\lambda & 0 \\ 2 & 2-\lambda \end{array} \\
&= (1-\lambda)(2-\lambda)(-\lambda)(-3)(-1)(1)(1-\lambda) \\
&= (1-\lambda)[(2-\lambda)(-\lambda)-3] = (1-\lambda)[\lambda^2-2\lambda-3] \\
&= PA(\lambda) \\
PA(\lambda) \stackrel{!}{=} 0 \quad & (1-\lambda)[\lambda^2-2\lambda-3] \stackrel{!}{=} 0 \\
& \lambda_1 = 1 \\
& \lambda_{2/3} = \frac{2 \pm \sqrt{4+12}}{2} = 1 \pm 2 \\
& \lambda_2 = 3 \quad \lambda_3 = -1
\end{align*}
\]

<|ref|>equation<|/ref|><|det|>[[135, 384, 560, 512]]<|/det|>
\[
\begin{align*}
\vec{E}_1 \text{ and } \lambda_1 &= 1 : \\
\begin{bmatrix}
0 & 0 & 0 \\
2 & 1 & -1 \\
0 & -3 & -1
\end{bmatrix}
&
\begin{bmatrix}
0 & 2 & 1 & -1 \\
0 & -3 & -1 & 0 \\
0 & 0 & 0 & 0
\end{bmatrix}
\\
-3y - z = 0 \iff y = -\frac{4}{3}z \quad \text{sette } z = t \\
2x + y - z = 0 \iff x = -\frac{4}{3}y + \frac{4}{3}z = \frac{4}{6}z + \frac{4}{6}z \\
\implies \vec{E}_1 = t \cdot \begin{pmatrix} 2 \\ -1 \\ 3 \end{pmatrix}
\end{align*}
\]

<|ref|>equation<|/ref|><|det|>[[135, 520, 647, 604]]<|/det|>
\[
\begin{align*}
\vec{E}_2 \text{ and } \lambda_2 &= 3 : \\
\begin{bmatrix}
-2 & 0 & 0 \\
2 & -1 & -1 \\
0 & -3 & -3
\end{bmatrix}
&
\begin{bmatrix}
0 & 2 & -1 & -1 \\
0 & -2 & 0 & 0 \\
0 & -3 & -3 & 0
\end{bmatrix}
&
\begin{bmatrix}
0 & 0 & 1 \\
0 & 1 & 1
\end{bmatrix}
\\
\implies \vec{E}_2 = t \cdot \begin{pmatrix} 3 \\ 1 \\ 1 \end{pmatrix}
\end{align*}
\]

<|ref|>equation<|/ref|><|det|>[[135, 621, 644, 816]]<|/det|>
\[
\begin{align*}
\vec{E}_3 \text{ and } \lambda_3 &= 3 : \\
\begin{bmatrix}
-2 & 0 & 0 \\
2 & 1 & -1 \\
0 & -3
\end{bmatrix}
&
\begin{bmatrix}
0 & 2 & -1 \\
0 & -2 & 0 \\
0 & -3
\end{bmatrix}
&
\begin{bmatrix}
0 & 0 & 1 \\
0 & -1 & 1 \\
0 & 0 & 0
\end{bmatrix}
\\
\implies \vec{E}_3 = t \cdot \begin{pmatrix} 3 \\ 1 \\ 1 \end{pmatrix} \\
\end{align*}
\]

<|ref|>equation<|/ref|><|det|>[[135, 831, 650, 919]]<|/det|>
\[
\begin{align*}
-y - z = 0 \iff y = -z \quad \text{sette } z = t \\
\lambda x - y - z = 0 \iff x = \frac{1}{2}y + \frac{1}{2}z = -\frac{1}{2}z + \frac{1}{2}z = 0 \\
\vec{E}_2 = t \cdot \begin{pmatrix} 0 \\ -1 \\ 1 \end{pmatrix}
\end{align*}
\]