<|ref|>equation<|/ref|><|det|>[[140, 85, 333, 115]]<|/det|>
\[ \vec{E}_3 \text{ auf } \vec{n}_3 = -1: \]

<|ref|>equation<|/ref|><|det|>[[150, 120, 608, 203]]<|/det|>
\[ \begin{array}{c|cc} \vec{z} & 0 & 0 \\ \hline \vec{z} & 3 & -1 \\ 0 & -3 & 1 \end{array} \quad \begin{array}{c|cc} \vec{z} & 3 & -1 \\ \hline 0 & 0 & 0 \\ 0 & -3 & 1 \end{array} \quad \begin{array}{cc} \vec{z} & 3 & -1 \\ \hline 0 & 1 & 0 \\ 0 & -3 & 1 \end{array} \]

<|ref|>equation<|/ref|><|det|>[[150, 212, 305, 295]]<|/det|>
\[ \begin{array}{c|cc} \vec{z} & 3 & -1 \\ 0 & -3 & 1 \\ 0 & -3 & 1 \end{array} \]

<|ref|>equation<|/ref|><|det|> [[150, 310, 699, 395]]<|/det|>
\[ \begin{array}{c} -3y + z = 0 \Leftrightarrow y = \frac{2}{3}z \quad \text{sohe} \quad z = t \\ 2x + 3y - z = 0 \Leftrightarrow x = -\frac{3}{2}y + \frac{2}{3}z = -\frac{2}{3}z + \frac{2}{3}z = 0 \\ \vec{E}_3 = t \cdot \begin{pmatrix} 0 \\ 3 \end{pmatrix} \end{array} \]

<|ref|>equation<|/ref|><|det|>[[120, 394, 644, 500]]<|/det|>
\[ f) \quad \det \left[ \begin{pmatrix} 2 & 1 & 0 \\ 0 & -2 & 1 \\ 1 & 0 & -2 \end{pmatrix} \right] = -2^3 + 1 = P_4(2) \]

<|ref|>equation<|/ref|><|det|>[[170, 465, 598, 515]]<|/det|>
\[ P_4(2) = 0 \Leftrightarrow -2^3 + 1 = 0 \quad \lambda^3 = 1 \]

<|ref|>equation<|/ref|><|det|>[[445, 516, 653, 540]]<|/det|>
\[ \lambda = 1 \]

<|ref|>equation<|/ref|><|det|>[[160, 550, 320, 580]]<|/det|>
\[ \vec{E}_1 \text{ auf } \vec{n} = 1: \]

<|ref|>equation<|/ref|><|det|>[[160, 580, 510, 655]]<|/det|>
\[ \begin{array}{c|cc} -1 & 1 & 0 \\ \hline 0 & -1 & 1 \\ 1 & 0 & -1 \end{array} \quad \begin{array}{c|cc} 0 & -1 & 1 \\ \hline 0 & 0 & 0 \\ 0 & 1 & -1 \end{array} \quad \begin{array}{c|cc} 0 \\ \hline 0 & 0 & 1 \\ 0 & 1 & -1 \end{array} \]

<|ref|>equation<|/ref|><|det|>[[160, 662, 585, 755]]<|/det|>
\[ \begin{array}{c} y - z = 0 \Leftrightarrow y = z \quad \text{sohe} \quad z = t \\ -x + y = 0 \Leftrightarrow x = y = z \\ \vec{E}_1 = t \cdot \begin{pmatrix} 1 \\ 1 \end{pmatrix} \end{array} \]