<|ref|>equation<|/ref|><|det|>[[145, 88, 480, 130]]<|/det|>
\[ \operatorname{tr}(\mathbb{1}) = \operatorname{tr}\left(\begin{bmatrix} 1 & 0 \\ 0 & 1 \end{bmatrix}\right) = 1 + 1 = \underline{2} \]

<|ref|>equation<|/ref|><|det|>[[135, 142, 630, 185]]<|/det|>
\[ \operatorname{det}(\mathbb{1}) = \operatorname{det}\left(\begin{bmatrix} 1 & 0 \\ 0 & 1 \end{ bmatrix}\right) = 1 \cdot 1 - 0 \cdot 0 = 1 - 0 = \underline{1} \]

<|ref|>equation<|/ref|><|det|>[[145, 196, 500, 240]]<|/det|>
\[ \operatorname{tr}(\hat{\mathbb{1}}) = \operatorname{tr}\left(\begin{bmatrix} 0 & -1 \\ 1 & 0 \end{bmatrix}\right) = 0 + 0 = \underline{0} \]

<|ref|>equation<|/ref|><|det|>[[145, 250, 681, 293]]<|/det|>
\[ \operatorname{det}(\hat{\mathbb{1}}) = \operatorname{det}\left(\begin{bmatrix} 0 & -1 \\ 1 & 0 \end{ bmatrix}\right) = 0 \cdot 0 - 1 \cdot (-1) = 0 + 1 = \underline{1} \]

<|ref|>equation<|/ref|><|det|>[[145, 304, 586, 347]]<|/det|>
\[ \operatorname{tr}(P) = \operatorname{tr}\left(\begin{bmatrix} -1 & 0 \\ 0 & -1 \end{bmatrix}\right) = -1 + (-1) = -\underline{2} \]

<|ref|>equation<|/ref|><|det|>[[130, 357, 732, 400]]<|/det|>
\[ \operatorname{det}(P) = \operatorname{det}\left(\begin{bmatrix} -1 & 0 \\ 0 & -1 \end{ bmatrix}\right) = (-1) \cdot (-1) - 0 \cdot 0 = 1 - 0 = \underline{1} = \underline{1} \]

<|ref|>equation<|/ref|><|det|>[[145, 401, 510, 444]]<|/det|>
\[ \operatorname{tr}(Z_{\lambda}) = \operatorname{tr}\left(\begin{bmatrix} \lambda & 0 \\ 0 & \lambda \end{bmatrix}\right) = \lambda + \lambda = 2\lambda \]

<|ref|>equation<|/ref|><|det|>[[130, 455, 664, 498]]<|/det|>
\[ \operatorname{det}(Z_{\lambda}) = \operatorname{det}\left(\begin{bmatrix} \lambda & 0 \\ 0 & \lambda \end{ bmatrix}\right) = \lambda \cdot \lambda - 0 \cdot 0 = \lambda^2 - 0 = \underline{\lambda^2} \]

<|ref|>equation<|/ref|><|det|>[[145, 508, 490, 551]]<|/det|>
\[ \operatorname{tr}(P_x) = \operatorname{tr}\left(\begin{bmatrix} 1 & 0 \\ 0 \end{bmatrix}\right) = 1 + 0 = \underline{1} \]

<|ref|>equation<|/ref|><|det|>[[130, 562, 636, 605]]<|/det|>
\[ \operatorname{det}(P_x) = \operatorname{det}\left(\begin{bmatrix} 1 & 0 \\ 0 \end{bmatrix}\right)= 1 \cdot 0 - 0 \cdot 0 = 0 - 0 = \underline{0} \]

<|ref|>equation<|/ref|><|det|>[[145, 616, 490, 660]]<|/det|>
\[ \operatorname{tr}(P_y) = \operatorname{tr}\left(\begin{bmatrix} 0 & 0 \\ 0 & 1 \end{bmatrix}\right) = 0 + 1 = \underline{1} \]

<|ref|>equation<|/ref|><|det|> [[130, 671, 636, 714]]<|/det|>
\[ \operatorname{det}(P_y) = \operatorname{det}\left(\begin{bmatrix} 0 & 0 \\ 0 & 1 \end{ bmatrix}\right) = 0 \cdot 1 - 0 \cdot 0 = 0 - 0 = \underline{0} = \underline{0} \]

<|ref|>equation<|/ref|><|det|>[[145, 725, 542, 768]]<|/det|>
\[ \operatorname{tr}(S_x) = \operatorname{tr}\left(\begin{bmatrix} 1 & 0 \\ -1 & 0 \end{bmatrix}\right) = 1 + (-1) = \underline{0} \]

<|ref|>equation<|/ref|><|det|>[[130, 779, 721, 822]]<|/det|>
\[ \operatorname{det}(S_x) = \operatorname{det}\left(\begin{bmatrix} 1 & 0 \\ -1 & 0 \end{ bmatrix}\right) = 1 \cdot (-1) - 0 \cdot 0 = -1 - 0 = -\underline{1} \]