<|ref|>text<|/ref|><|det|>[[114, 81, 815, 101]]<|/det|>
a) \(C = A + B\) b) \(C = -2A\) c) \(C = B/3\) d) \(C = 2B - A\) 

<|ref|>equation<|/ref|><|det|>[[255, 113, 741, 150]]<|/det|>
\[D = \begin{pmatrix} 3 & 2 & 5 \\ -1 & 2 & 3 \end{pmatrix}, E = \begin{pmatrix} 1 & 8 & -2 \\ 3 & 0 & 1 \end{pmatrix}, F = \begin{pmatrix} 5 & 0 & 10 \\ 0 & -2 & 8 \end{pmatrix}\]

<|ref|>text<|/ref|><|det|>[[114, 153, 682, 172]]<|/det|>
e) \(D + E + F\) f) \(3D - 2(E + 5F)\) g) \(3D^T - 3(E + 2F)^T\) 

<|ref|>text<|/ref|><|det|>[[114, 171, 475, 189]]<|/det|>
h) \(2(D + E) - 3(D^T - E^T)^T + 5(F - 2D)\) 

<|ref|>text<|/ref|><|det|>[[114, 205, 144, 220]]<|/det|>
a) 

<|ref|>equation<|/ref|><|det|>[[120, 225, 839, 319]]<|/det|>
\[ \begin{aligned} \underline{C} &= A + B = \begin{bmatrix} 1 & 3 & -1 \\ 4 & -2 & 8 \end{bmatrix} + \begin{bmatrix} -3 & 9 & 3 \\ -6 & 6 & 3 \end{bmatrix} = \begin{bmatrix} 1 + (-3) & 3 + 9 & -1 + 3 \\ 4 + (-6) & -2 + 6 & 8 + 3 \end{bmatrix} \\ &= \begin{bmatrix} -2 & 12 & 2 \\ -2 & 4 & 11 \end{bmatrix}. \end{aligned} \]

<|ref|>text<|/ref|><|det|>[[114, 323, 144, 339]]<|/det|>
b) 

<|ref|>equation<|/ref|><|det|>[[114, 339, 792, 384]]<|/det|>
\[ \underline{C} = -2 \cdot A = \begin{bmatrix} (-2) \cdot 1 & (-2) \cdot 3 & (-2) \cdot (-1) \\ (-2) \cdot 4 & (-2) \cdot (-2) & (-2) \cdot 8 \end{bmatrix} = \begin{bmatrix} -2 & -6 & 2 \\ -8 & 4 & -16 \end{bmatrix}. \]

<|ref|>text<|/ref|><|det|>[[114, 389, 144, 405]]<|/det|>
c) 

<|ref|>equation<|/ref|><|det|>[[128, 408, 515, 480]]<|/det|>
\[ \underline{C} = \frac{B}{3} = \begin{bmatrix} -3 & 9 & 3 \\ 3 & 3 & 3 \\ -6 & 6 & 3 \\ 3 & 3 & 3 \end{bmatrix} = \begin{bmatrix} -1 & 3 & 1 \\ -2 & 2 & 1 \end{bmatrix} \]

<|ref|>text<|/ref|><|det|>[[114, 480, 144, 496]]<|/det|>
d) 

<|ref|>equation<|/ref|><|det|>[[114, 496, 844, 542]]<|/det|>
\[ \underline{C} = 2 \cdot B - A = \begin{bmatrix} 2 \cdot (-3) - 1 & 2 \cdot 9 - 3 & 2 \cdot 3 - (-1) \\ 2 \cdot (-6) - 4 & 2 \cdot 6 - (-2) & 2 \cdot 3 - 8 \end{bmatrix} = \begin{bmatrix} -7 & 15 & 7 \\ -16 & 14 & -2 \end{bmatrix} \]

<|ref|>text<|/ref|><|det|>[[114, 547, 144, 563]]<|/det|>
e) 

<|ref|>equation<|/ref|><|det|>[[118, 567, 717, 612]]<|/det|>
\[ \begin{pmatrix} 3 + 1 + 5 & 2 + 8 + 0 & 5 - 2 + 10 \\ -1 + 3 + 0 & 2 + 0 - 2 & 3 + 1 + 8 \end{pmatrix} = \begin{pmatrix} 9 & 10 & 13 \\ 2 & 0 & 12 \end{pmatrix} \]

<|ref|>text<|/ref|><|det|>[[114, 613, 140, 629]]<|/det|>
f) 

<|ref|>equation<|/ref|><|det|>[[118, 632, 323, 675]]<|/det|>
\[ \begin{pmatrix} -43 & -10 & -81 \\ -9 & 26 & -73 \end{pmatrix} \]

<|ref|>text<|/ref|><|det|>[[114, 678, 140, 694]]<|/det|>
g) 

<|ref|>equation<|/ref|><|det|>[[118, 697, 260, 762]]<|/det|>
\[ \begin{pmatrix} -35 & -15 \\ -26 & 22 \\ -57 & -59 \end{pmatrix} \]

<|ref|>text<|/ref|><|det|>[[114, 766, 140, 782]]<|/det|>
h) 

<|ref|>equation<|/ref|><|det|>[[118, 782, 308, 825]]<|/det|>
\[ \begin{pmatrix} -3 & 18 & -15 \\ 26 & -32 & 12 \end{pmatrix} \]