Bsp: a) $f(x)=2 x \cdot \operatorname{en} x$

$$
\begin{aligned}
f^{\prime}(x) & =2 \cdot \operatorname{en} x+2 x \cdot \frac{1}{x}=2 \cdot \operatorname{en} x+2 x \cdot x^{-1} \\
& =2 \cdot \operatorname{en} x+2 x^{\circ}=2 \operatorname{en} x+2 \\
f^{\prime \prime}(x) & =2 \cdot \frac{1}{x}=\frac{2}{x}
\end{aligned}
$$

b) $f(x)=x^{n} \cdot e^{x}$

$$
\begin{aligned}
f^{\prime}(x) & =n \cdot x^{n-1} \cdot e^{x}+x^{n} \cdot e^{x} \\
& =x^{n-1} \cdot e^{x} \cdot(n+1) \\
f^{\prime \prime}(x) & =(n-1) \cdot x^{n-2} \cdot e^{x} \cdot(n+x)+x^{n-1} \cdot\left[e^{x}(n+1)+e^{x} \cdot 1\right] \\
& =(n-1) \cdot x^{n-2} \cdot e^{x}(n+x)+x^{n-1} \cdot e^{x}(n+1)+x^{n-1} \cdot e^{x} \\
& =x^{n-2} \cdot e^{x} \cdot[-(n-1)(n+x)+x \cdot(n+x)+x]
\end{aligned}
$$

c) $f(x)=\underbrace{\left(x^{2}-1\right)^{2}}_{2\left(x^{2}-1\right) \cdot 2 x} \cdot \underbrace{(x+5)^{3}}_{3(x+5)^{2} \cdot 1}$

$$
\begin{aligned}
f^{\prime}(x) & =4 x\left(x^{2}-1\right) \cdot(x+5)^{3}+\left(x^{2}-1\right)^{2} \cdot 3(x+5)^{2} \\
& =\left(x^{2}-1\right)(x+5)^{2} \cdot\left[4 x \cdot(x+5)+3 \cdot\left(x^{2}-1\right)\right] \\
& =\left(x^{2}-1\right)(x+5)^{2} \cdot\left[4 x^{2}+20 x+3 x^{2}-3\right] \\
& =\left(x^{2}-1\right)(x+5)^{2} \cdot\left[7 x^{2}+20 x-3\right]
\end{aligned}
$$