# Ableitung mittels Differenzquotient: 

$$
\begin{aligned}
& f(x)=x^{2} \\
& \frac{\Delta y}{\Delta x}=\frac{f(x+\Delta x)-f(x)}{\Delta x}=\frac{(x+\Delta x)^{2}-x^{2}}{\Delta x} \\
& =\frac{x^{2}+2 \cdot \Delta x \cdot x+\Delta x^{2}-x^{2}}{\Delta x}=\frac{2 \Delta x \cdot x+\Delta x^{2}}{\Delta x}=\frac{\Delta x(2 x+\Delta x)}{\Delta x}=2 x+\Delta x \\
& f^{\prime}(x)=\lim _{\Delta x \rightarrow 0} \frac{\Delta y}{\Delta x}=\lim _{\Delta x \rightarrow 0}(2 x+\Delta x)=2 x \\
& \rightarrow f(x)=x^{2}, f^{\prime}(x)=2 x
\end{aligned}
$$

## Monom - Regel:

$$
\begin{aligned}
& f: A \subseteq \mathbb{R} \rightarrow \mathbb{R}, f(x)=x^{p} \quad \text { mit } p \in \mathbb{R} \backslash \mathbb{E O} \text {; } \\
& f^{\prime}(x)=p \cdot x^{p-1}
\end{aligned}
$$

## Bep:

- $f(x)=x^{5}$

$$
f^{\prime}(x)=5 \cdot x^{4}
$$

- $f(x)=\frac{1}{x}=x^{-1}$
$f^{\prime}(x)=-x^{-2}=-\frac{1}{x^{2}}$
- $f(x)=\sqrt{x}=x^{\pi / 2}$
$f^{\prime}(x)=\frac{1}{2} x^{\pi / 2-1}=\frac{1}{2} x^{-\pi / 2}=\frac{1}{2} \frac{1}{x^{2 / 2}}=\frac{1}{2 \cdot \sqrt{x^{2}}}$

Regeln:

- $f(x)=a \cdot g(x)$
$f^{\prime}(x)=a \cdot g^{\prime}(x)$
$f(x)=g(x)+h(x)$
$f^{\prime}(x)=g^{\prime}(x)+h^{\prime}(x)$
$f(x)=a^{\prime}(x)+h^{\prime}(x)$
$f(x)=5 \cdot x^{4}$
$f(x)=x^{-1}$
$f^{\prime}(x)=-x^{-2}=-\frac{1}{x^{2}}$
- $f(x)=\sqrt{x}=x^{\pi / 2}$
$f^{\prime}(x)=\frac{1}{2} x^{\pi / 2-1}=\frac{1}{2} x^{-\pi / 2}=\frac{1}{2} \frac{1}{x^{2 / 2}}=\frac{1}{2 \cdot \sqrt{x^{2}}}$


## $\int$ Summenregel