<|ref|>text<|/ref|><|det|>[[20, 0, 84, 42]]<|/det|>
A3 

<|ref|>text<|/ref|><|det|>[[20, 50, 604, 90]]<|/det|>
a) \(x u_x + y u_y + (x^2 + y^2) u = 0\) 

<|ref|>equation<|/ref|><|det|>[[95, 87, 430, 140]]<|/det|>
\[u(x, -x^2) = e^{-\frac{x^2}{2}}\]

<|ref|>equation<|/ref|><|det|>[[767, 53, 870, 131]]<|/det|>
\[PDE\]

<|ref|>equation<|/ref|><|det|>[[767, 99, 860, 133]]<|/det|>
\[CE\]

<|ref|>equation<|/ref|><|det|>[[95, 155, 978, 220]]<|/det|>
\[x \frac{\partial u(x,y)}{\partial x} + y \frac{\partial u(x,y)}{\partial y} + (x^2 + y^2) u(x,y) = 0 \quad PDE\]

<|ref|>text<|/ref|><|det|>[[10, 245, 861, 333]]<|/det|>
**Commutativit√§t:**
\[< \vec{a}'(x', u(x'))>, \quad \nabla u(x') >\]
\[+ b(x', u(x')) = 0\]

<|ref|>equation<|/ref|><|det|>[[40, 333, 960, 440]]<|/det|>
\[\vec{a} = \begin{pmatrix} x \\ y \end{pmatrix} = \vec{k} \begin{pmatrix} 1 \\ 0 \end{pmatrix} \quad w(s) = u(\vec{k} \begin{pmatrix} 1 \\ 0 \end{pmatrix})\]

<|ref|>equation<|/ref|><|det|>[[560, 400, 960, 490]]<|/det|>
\[w'(s) = < \nabla u, \vec{k} \begin{pmatrix} 1 \\ 0 \end{pmatrix} >\]

<|ref|>equation<|/ref|><|det|>[[20, 480, 960, 572]]<|/det|>
\[\rightarrow \vec{a} = \vec{k} \begin{pmatrix} 1 \\ 0 \end{pmatrix} = \begin{pmatrix} k_1(s) \\ k_2(s) \end{pmatrix} = \begin{pmatrix} k_1'(s) \\ k_2'(s) \end{pmatrix} \quad (1)\]

<|ref|>equation<|/ref|><|det|>[[40, 592, 740, 636]]<|/det|>
\[w'(s) = -(k_1^2 + k_2^2) w(s) \quad (2)\]

<|ref|>text<|/ref|><|det|>[[0, 657, 710, 750]]<|/det|>
**aus (1) und (2):**
\(k_1(s) = c_1 \cdot e^s\)
\(k_2(s) = c_2 \cdot e^s\) 

<|ref|>text<|/ref|><|det|>[[10, 760, 768, 810]]<|/det|>
**aus (3):**
\(w'(s) = -e^{2s}(c_1^2 + c_2^2) w(s)\) 

<|ref|>equation<|/ref|><|det|>[[175, 810, 742, 867]]<|/det|>
\[\frac{1}{w(s)} \frac{dw}{ds} = -e^{2s}(c_1^2 + c_2^2)\]

<|ref|>equation<|/ref|><|det|>[[185, 884, 816, 980]]<|/det|>
\[\ln |w| = -\frac{1}{2} e^{2s}(c_1^2 + c_2^2) + c_3\]

<|ref|>equation<|/ref|><|det|>[[910, 963, 975, 998]]<|/det|>
\[\circledcirc\]