<|ref|>equation<|/ref|><|det|>[[192, 85, 525, 265]]<|/det|>
\[
\begin{align*}
a_1 &= \frac{2}{\pi} \int_0^\pi f(x) \cos x \, dx \\
&= \frac{2}{\pi} \int_0^{\pi/2} x \cos x \, dx + \frac{2}{\pi} \int_{\pi/2}^\pi \cos x \, dx \\
&= \frac{2}{\pi} \left[ x \sin x + \cos x \right]_0^{\pi/2} + \left[ \sin x \right]_{\pi/2}^{\pi} \\
&= 1 - \frac{2}{\pi} - 1 = -\frac{2}{\pi}.
\end{align*}
\]

<|ref|>text<|/ref|><|det|>[[119, 274, 480, 293]]<|/det|>
Da \(f_a\) reell und gerade sein soll, ist \(b_1 = 0\) und 

<|ref|>equation<|/ref|><|det|>[[266, 305, 453, 338]]<|/det|>
\[
c_1 = c_{-1} = \frac{a_1}{2} = -\frac{1}{\pi}.
\]

<|ref|>text<|/ref|><|det|>[[115, 341, 150, 359]]<|/det|>
b) 

<|ref|>text<|/ref|><|det|>[[115, 357, 560, 377]]<|/det|>
Da f ungerade ist, gilt: \(c_0 = a_0 = 0\) und \(a_1 = 0\). 

<|ref|>image<|/ref|><|det|>[[115, 375, 710, 784]]<|/det|>