<|ref|>text<|/ref|><|det|>[[120, 84, 250, 110]]<|/det|>
6) \(j \neq k\): 

<|ref|>equation<|/ref|><|det|>[[160, 108, 419, 139]]<|/det|>
\[0 \subset_+ = 1; \quad \subset_- = 1\]

<|ref|>equation<|/ref|><|det|>[[180, 145, 692, 179]]<|/det|>
\[j+k = 4m_1 \land j-k = 4m_2 \quad m \in \mathbb{N}\]

<|ref|>text<|/ref|><|det|>[[120, 185, 242, 211]]<|/det|>
7) \(j \neq k\): 

<|ref|>equation<|/ref|><|det|>[[160, 209, 760, 283]]<|/det|>
\[0 \subset_+ = 0 \implies j+k \text{ ungarneale} \implies j-k \text{ ungarneale} \\ \implies S = -\frac{1}{2} \left( \frac{-2j}{j^2-k^2} \right) \neq 0\]

<|ref|>text<|/ref|><|det|>[[120, 295, 234, 321]]<|/det|>
8) \(j \neq k\) 

<|ref|>equation<|/ref|><|det|>[[160, 320, 707, 450]]<|/det|>
\[0 \subset_+ = -1 \quad j+k = 2+4m \quad m \in \mathbb{N} \\ \rightarrow \text{Stiller:} \quad -j+k + C_+ (j+k) - 2j = 0 \\ \quad -3j+k = -C_+ (j+k) \\ \quad -4j+j+k = C_+ (j+k)\]

<|ref|>text<|/ref|><|det|>[[120, 468, 565, 499]]<|/det|>
0. dumi \(S = 0\) gül für \(C_+ = -1\): 

<|ref|>equation<|/ref|><|det|>[[150, 504, 700, 560]]<|/det|>
\[\text{Stiller:} \quad -3j+k = 1(j+k) \\ \quad -4j = 0 \quad \text{mit möglich}\]

<|ref|>text<|/ref|><|det|>[[120, 580, 512, 610]]<|/det|>
0. dumi \(S = 0\) für \(C_+ = 0\): 

<|ref|>equation<|/ref|><|det|>[[150, 614, 520, 690]]<|/det|>
\[\text{Stiller:} \quad -j+k - 2j = 0 \\ \quad +3j = k \\ \quad \text{Unwasssetzung:} \quad k = 2+4m-j \\ \quad 3j+j = 2+4m \\ \quad j = \frac{1}{2} + m\]

<|ref|>equation<|/ref|><|det|>[[275, 694, 750, 730]]<|/det|>
\[\text{unseren:} \quad C_+ = 0 \implies \cos((j-k)\frac{\pi}{2})\]

<|ref|>equation<|/ref|><|det|>[[275, 735, 755, 770]]<|/det|>
\[j-k = 1+2m \quad m \in \mathbb{N}\]

<|ref|>equation<|/ref|><|det|>[[275, 767, 570, 793]]<|/det|>
\[\text{unseren von } 3j = k\]

<|ref|>equation<|/ref|><|det|>[[275, 792, 633, 828]]<|/det|>
\[j - 3j = 1+2m\]

<|ref|>equation<|/ref|><|det|>[[275, 825, 656, 860]]<|/det|>
\[-2j = 1+2m\]

<|ref|>equation<|/ref|><|det|>[[275, 856, 656, 892]]<|/det|>
\[< 0 \quad > 0\]