<|ref|>equation<|/ref|><|det|>[[68, 0, 777, 150]]<|/det|>
\[
\begin{align*}
v'(x) &= c_1 \sqrt{k} e^{\sqrt{k}x} - c_2 \sqrt{k} e^{-\sqrt{k}x} \\
v''(x) &= c_1 k e^{\sqrt{k}x} + c_2 k e^{-\sqrt{k}x} \\
\text{while } w(y) &= c_3 e^{\sqrt{k}y} + c_4 e^{-\sqrt{k}y}
\end{align*}
\]

<|ref|>equation<|/ref|><|det|>[[10, 178, 748, 255]]<|/det|>
\[
\text{IC: } v(0, y) = v(0) \cdot w(y) = v(1) \cdot w(y) = 0 \\
v(0) = v(1) = 0
\]

<|ref|>equation<|/ref|><|det|>[[100, 259, 844, 312]]<|/det|>
\[
v(0) = c_1 + c_2 = c_1 e^{\sqrt{k}} + c_2 e^{-\sqrt{k}} = 0
\]

<|ref|>equation<|/ref|><|det|>[[50, 325, 650, 640]]<|/det|>
\[
\begin{align*}
&\rightarrow c_1 = -c_2 \\
&\rightarrow c_1 e^{\sqrt{k}} - c_1 e^{-\sqrt{k}} = 0 \\
&\quad c_1 \cdot (e^{\sqrt{k}} - e^{-\sqrt{k}}) = 0 \\
&\quad e^{\sqrt{k}} = e^{-\sqrt{k}} \\
&\quad e^{2\sqrt{k}} = 1 \\
&\quad 2\sqrt{k} = 2\pi i \cdot n \\
&\quad k = -\sqrt{n^2} n^2
\end{align*}
\]

<|ref|>equation<|/ref|><|det|>[[10, 670, 920, 970]]<|/det|>
\[
\text{as originally stated, then } w(y): \\
w(y) = c_3 e^{\sqrt{-\sqrt{n^2}n^2}y} + c_4 e^{-\sqrt{-\sqrt{n^2}n^2}y}
\]

<|ref|>equation<|/ref|><|det|>[[855, 963, 900, 995]]<|/det|>
\[
\circled{2}
\]