<|ref|>equation<|/ref|><|det|>[[25, 0, 920, 150]]<|/det|>
\[
\begin{align*}
b) \quad & \pm U_t + U_x = 2U \quad & u(x,t) \\
& \pm \frac{\partial u(x,t)}{\partial t} + \frac{\partial u(x,t)}{\partial x} - 2u = 0 \quad & \text{BC} \\
& u(x,1) = x \quad & \text{CC} \\
& \text{Remark:} \quad & \vec{a} = \begin{pmatrix} 1 \\ t \end{pmatrix} = \vec{k}'(s) \\
& w(s) = u(\vec{k}'(s)) \quad & \\
& w'(s) = 2 \cdot w(s) \quad & \\
& \Rightarrow \quad & \\
& k_1'(s) = 1 \quad & k_1(s) = 5 + c_1 \quad (1) \\
& k_2'(s) = t = k_2(s) \quad & k_2(s) = c_2 \cdot e^s \quad (2) \\
& w'(s) = 2 \cdot w(s) \quad & \iff \quad \frac{dw}{w} = 2 \quad \text{ds} \\
& \quad & \ln |w| = 2s + c_3 \quad (3) \\
& \quad & w = e^{2s} \cdot e^{c_3} = c_3 \cdot e^{2s} \quad (3) \\
\end{align*}
\]

<|ref|>equation<|/ref|><|det|>[[18, 150, 999, 900]]<|/det|>
\[
\begin{align*}
\text{Remark:} \quad & \vec{a} = \begin{pmatrix} 1 \\ \vec{k}'(s) \end{pmatrix} = \vec{k}'(s) \\
& w(s) = u\left(\vec{k}'(s)\right) \\
& w'(s) = 2 \cdot w(s) \\
& \Rightarrow \quad & \\
& k_1'(s) = 1 \qquad k_1(s) = 5 + c_1 \qquad (1) \\
& k_2'(s) = t = k_2(s) & k_2(s) = c_2 \cdot e^s \qquad (2) \\
& w'(s) = 2 \cdot w(s) \quad \iff \quad \frac{dw}{w} = 2 \quad \text{ ds} \\
& \quad & \ln |w| = 2s + c_3 \\
& \quad & w = e^{2s} \cdot e^{c_3}=c_3 \cdot e^{2s} \qquad (3) \\
& \quad & w = e^{2s} \cdot e^{2s} = c_3 \cdot e^{2s} \qquad (3) \\
& \quad & \text{Remark:} \quad & \vec{a} = \begin{pmatrix} 2 \\ \vec{k}'(s) \end{pmatrix} = \vec{k}'(s)
\end{align*}
\]

<|ref|>equation<|/ref|><|det|>[[0, 0, 999, 999]]<|/det|>
\[
\begin{align*}
\text{Remark:} \quad & \vec{a}=\begin{pmatrix} 1 \\ \vec{k}'(s) \end{pmatrix}=\vec{k}'(s) \\
& w(s)=u(\vec{k}'(s)) \\
& w'(s)=2\cdot w(s) \\
& \Rightarrow \quad & \\
& k_1'(s)=1 \qquad k_1(s)=5+c_1 \qquad (1) \\
& k_2'(s)=t=k_2(s) \qquad k_2(s)=c_2\cdot e^s \qquad (2) \\
& w'(s)=2\cdot w(s) \quad \iff \quad \frac{dw}{w}=2 \quad \text{ds} \\
& \quad & \ln|w|=2s+c_3 \qquad (3) \\
& \quad & w=e^{2s}\cdot e^{c_3}=c_3\cdot e^{2s} \qquad (3) \\
& \quad & \text{Remark} \quad & \vec{a}=\begin{pmatrix} 2 \\ \vec{k}'(s) \end{pmatrix}=\vec{k}'(s)
\end{align*}
\]

\[
\begin{align*}
\text{Remark:} \quad & \vec{a}=\begin{pmatrix}\vec{k}'(s)\end{pmatrix}=\vec{k}'(s) \\
& w(s)=u(\vec{k}''(s)) \\
& w'(s)=2\cdot w(s) \\
& \Rightarrow \quad \frac{dw}{w}=2 \quad \text{ds} \\
& w=2s+c_3 \qquad (3) \\
& w=e^{2s}\cdot e^{c_3}=c_3\cdot e^{s} \qquad (3) \\
& \text{Remark} \quad & \vec{a}=\begin{pmatrix} 2 \\ \frac{\vec{k}'(s)}{w} \end{pmatrix}=\frac{\vec{k}'(s)}{w}
\end{align*}
\]

\[
\begin{align*}
\text{Remark:} \quad & \vec{\alpha}=\begin{pmatrix} 1 \\ \vec{k}'(s) \end{pmatrix}=\vec{\alpha}'(s) \\
& w(s)=u(\vec{\alpha}'(s)) \\
& w'(s)=2\cdot w(s) \\
& \Rightarrow\quad \frac{dw}{w}=2 \quad \text{ds} \\
& w=1+2s+c_3 \qquad (3) \\
& w=e^{2s}\cdot c_3=e^{2s}\cdot 1 \qquad (3) \\
& \text{Remark} \quad & \vec{\alpha}=\begin{pmatrix} 2 \\ \vec{k}'(s) \end{pmatrix}=\vec{\alpha}'(s)
\end{align*}
\]

\[
\begin{align*}
\text{Remark:} \qquad \vec{\alpha}=\begin{pmatrix} 1 \\ \vec{k}'(s) \begin{pmatrix} 1 \\ \vec{k}'(s) \end{pmatrix} \end{pmatrix}=\vec{\alpha}'(s) \\
& w(s)=u(\vec{k}'(s)) \\
& \Rightarrow \quad \frac{dw}{w}=2 \quad \text{ ds} \\
& w=1+2s+c_3 \qquad (3) \\
& \text{Remark} \quad & \vec{\alpha} = \begin{pmatrix} 2 \\ \vec{k}'(s) \end{pmatrix}=\vec{\kappa}'(s)
\end{align*}
\]

\[
\begin{align*}
\text{Remark:} \vec{\alpha}=\begin{pmatrix} 1 \\ \vec{k}'(s) \vec{\alpha} \end{pmatrix}=\vec{\alpha}'(s) \\
& w(s)=u(\begin{pmatrix} 1 \\ \vec{k}'(s) \end{pmatrix}) \\
& \Rightarrow \quad \frac{dw}{w}=2 \quad \text{ d s} \\
& w=1+2s+c_3 \qquad (3) \\
& & \text{Remark} \quad & \vec{\alpha} = \begin{pmatrix} 1 \\ \vec{k}'(s) \end{pmatrix}=\vec{\kappa}'(s)
\