<|ref|>text<|/ref|><|det|>[[114, 84, 140, 100]]<|/det|>
a) 

<|ref|>equation<|/ref|><|det|>[[123, 103, 694, 150]]<|/det|>
\[ \mathcal{F}^{-1} \left\{ \frac{5}{(2 + \mathrm{j}\omega)^2} \right\} = 5 \cdot \mathcal{F}^{-1} \left\{ \frac{1}{(2 + \mathrm{j}\omega)^2} \right\} = 5 t \cdot \mathrm{e}^{-2t} \cdot \sigma(t) \]

<|ref|>text<|/ref|><|det|>[[114, 152, 140, 168]]<|/det|>
b) 

<|ref|>equation<|/ref|><|det|>[[121, 169, 756, 202]]<|/det|>
\[ \mathcal{F}^{-1} \left\{ \cos(5\omega) \right\} = \frac{1}{2} \cdot \mathcal{F}^{-1} \left\{ 2 \cdot \cos(5\omega) \right\} = \frac{1}{2} \left[ \delta(t+5) + \delta(t-5) \right] \]

<|ref|>text<|/ref|><|det|>[[114, 206, 140, 222]]<|/det|>
c) 

<|ref|>equation<|/ref|><|det|>[[123, 223, 813, 260]]<|/det|>
\[ F(\omega) = 2 \cdot \frac{1}{5 + \mathrm{j}\omega} - 3 \cdot \frac{1}{2 + \mathrm{j}\omega} \Rightarrow f(t) = (2 \cdot \mathrm{e}^{-5t} - 3 \cdot \mathrm{e}^{-2t}) \cdot \sigma(t) \]