<|ref|>equation<|/ref|><|det|>[[40, 9, 850, 150]]<|/det|>
\[
\begin{align*}
x &= k_1(S) = S + G_1 = S + \gamma \quad \iff \quad S = x - \gamma \\
L \triangle t &= k_2(S) = C_2 \cdot e^S = e^S = e^{x - \gamma} = \frac{e^x}{e^\gamma} \\
e^{\gamma t} &= \frac{e^x}{t} \quad \iff \quad \ln \frac{e^x}{t} = \gamma \\
\ln e^x - \ln t &= \gamma \\
\gamma = x - \ln t
\end{align*}
\]

<|ref|>equation<|/ref|><|det|>[[33, 275, 961, 520]]<|/det|>
\[
\begin{align*}
u(x,t) &= \gamma \cdot \frac{e^x}{e^\gamma} \cdot \frac{e^x}{e^\gamma} = (x - \ln t) \cdot \frac{e^{2x}}{e^{2(x - \ln t)}} \\
&= (x - \ln t) \cdot \frac{e^{2x}}{e^{2x} \cdot e^{-2 \ln t}} = (x - \ln t) \cdot e^{2 \ln t} \\
&= (x - \ln t) \cdot t^2
\end{align*}
\]