<|ref|>text<|/ref|><|det|>[[119, 82, 220, 99]]<|/det|>
Daraus folgt 

<|ref|>equation<|/ref|><|det|>[[249, 112, 469, 149]]<|/det|>
\[c_1 = -\frac{ib_1}{2} = -\mathrm{i}\left(\frac{1}{\pi} + \frac{1}{2}\right)\]

<|ref|>text<|/ref|><|det|>[[119, 162, 155, 176]]<|/det|>
und 

<|ref|>equation<|/ref|><|det|>[[253, 188, 463, 225]]<|/det|>
\[c_{-1} = \frac{ib_1}{2} = \mathrm{i}\left(\frac{1}{\pi} + \frac{1}{2}\cdot\right).\]

<|ref|>text<|/ref|><|det|>[[115, 224, 140, 241]]<|/det|>
c) 

<|ref|>text<|/ref|><|det|>[[144, 241, 234, 256]]<|/det|>
Es gilt hier 

<|ref|>equation<|/ref|><|det|>[[227, 268, 490, 373]]<|/det|>
\[c_0 = a_0 = \frac{1}{2\pi} \int_{-\pi}^{\pi} f(x) \, \mathrm{d}x \\
= \frac{2}{2\pi} \int_{0}^{\pi} f(x) \, \mathrm{d}x = \frac{3}{8} \pi\]

<|ref|>text<|/ref|><|det|>[[119, 382, 312, 397]]<|/det|>
wie in Teil (a). Ferner ist 

<|ref|>equation<|/ref|><|det|>[[148, 408, 568, 515]]<|/det|>
\[a_1 = \frac{1}{\pi} \int_{-\pi}^{\pi} f(x) \cos x \, \mathrm{d}x \\
= \frac{1}{\pi} \int_{-\pi}^{0} f(x + \pi) \cos x \, \mathrm{d}x + \frac{1}{\pi} \int_{0}^{\pi} f(x) \cos x \, \mathrm{d}x.\]

<|ref|>text<|/ref|><|det|>[[119, 525, 537, 542]]<|/det|>
Mit der Substitution \(t = x + \pi\) im ersten Integral folgt 

<|ref|>equation<|/ref|><|det|>[[153, 552, 562, 675]]<|/det|>
\[a_1 = \frac{1}{\pi} \int_{0}^{\pi} f(t) \cos(t - \pi) \, \mathrm{d}t + \frac{1}{\pi} \int_{0}^{\pi} f(x) \sin x \, \mathrm{d}x \\
= -\frac{1}{\pi} \int_{0}^{\pi} f(t) \cos(t) \, \mathrm{d}t + \frac{1}{\pi} \int_{0}^{\frac{\pi}{2}} f(x) \cos x \, \mathrm{d}x \\
= 0.\]

<|ref|>text<|/ref|><|det|>[[119, 690, 572, 706]]<|/det|>
und ganz analog folgt \(b_1 = 0\). Damit ist auch \(c_1 = c_{-1} = 0\).