<|ref|>text<|/ref|><|det|>[[20, 9, 245, 40]]<|/det|>
Darstellungen : 

<|ref|>text<|/ref|><|det|>[[50, 50, 728, 160]]<|/det|>
- Grundform : \(m\) und \(q\) gegeben, \(m, q \in \mathbb{R}\)
  \(f(x)\) l√§sst sich durch
  \(f(x) = m \cdot x + q\) darstellen 

<|ref|>text<|/ref|><|det|>[[20, 186, 400, 255]]<|/det|>
Bsp.: \(m = 5, q = -2\)
\(f(x) = 5x - 2\) 

<|ref|>text<|/ref|><|det|>[[50, 282, 640, 353]]<|/det|>
- Taylorform : \(m\) und \(P(x_0, y_0)\) gegeben
  \(\rightarrow f(x) = m(x - x_0) + y_0\) 

<|ref|>text<|/ref|><|det|>[[20, 380, 680, 490]]<|/det|>
Bsp.: \(m = 0,5\)
\(P(1; 3)\)
\(f(x) = 0,5(x - 1) + 3 = 0,5x - 0,5 + 3\)
\(= 0,5x + 2,5\) 

<|ref|>text<|/ref|><|det|>[[50, 517, 950, 666]]<|/det|>
- 2-Punkel - Form : \(2\) Punkte \(P_1(x_1, y_1)\) & \(P_2(x_2, y_2)\) gegeben
  \(\rightarrow m = \frac{y_2 - y_1}{x_2 - x_1}\)
  \(\rightarrow f(x) = m(x - x_1) + y_1\)
  \(= m(x - x_2) + y_2\) 

<|ref|>text<|/ref|><|det|>[[20, 692, 437, 720]]<|/det|>
Bsp.: \(P_1(1; 3)\)
\(P_2(4; 5)\) 

<|ref|>equation<|/ref|><|det|>[[163, 725, 666, 838]]<|/det|>
\[
\begin{align*}
m &= \frac{5 - 3}{4 - 1} = \frac{2}{3} \\
f(x) &= \frac{2}{3}(x - 1) + 3 = \frac{2}{3}x - \frac{2}{3} + 3 \\
&= \frac{2}{3}x + \frac{2}{3}
\end{align*}
\]