<|ref|>text<|/ref|><|det|>[[25, 10, 430, 40]]<|/det|>
Bsp: a) \(f(x) = 2x \cdot \text{en} x\) 

<|ref|>equation<|/ref|><|det|>[[183, 44, 870, 115]]<|/det|>
\[
\begin{align*}
f'(x) &= 2 \cdot \text{en} x + 2x \cdot \frac{1}{x} = 2 \cdot \text{en} x + 2x \cdot x^{-1} \\
&= 2 \cdot \text{en} x + 2x^0 = 2 \text{en} x + 2
\end{align*}
\]

<|ref|>equation<|/ref|><|det|>[[183, 120, 470, 161]]<|/det|>
\[
f''(x) = 2 \cdot \frac{1}{x} = \frac{2}{x}
\]

<|ref|>text<|/ref|><|det|>[[135, 184, 386, 215]]<|/det|>
b) \(f(x) = x^n \cdot e^x\) 

<|ref|>equation<|/ref|><|det|>[[183, 220, 627, 290]]<|/det|>
\[
\begin{align*}
f'(x) &= n \cdot x^{n-1} \cdot e^x + x^n \cdot e^x \\
&= x^{n-1} \cdot e^x \cdot (n+1)
\end{align*}
\]

<|ref|>equation<|/ref|><|det|>[[183, 297, 960, 410]]<|/det|>
\[
\begin{align*}
f''(x) &= (n-1) \cdot x^{n-2} \cdot e^x \cdot (n+x) + x^{n-1} \cdot [e^x(n+1) + e^x \cdot 1] \\
&= (n-1) \cdot x^{n-2} \cdot e^x \cdot(n+x) + x^{n-1} \cdot e^x(n+1) + x^{n-1} \cdot e^x \\
&= x^{n-2} \cdot e^x \cdot [(n-1)(n+x) + x \cdot (n+x) + x]
\end{align*}
\]

<|ref|>text<|/ref|><|det|>[[135, 435, 571, 470]]<|/det|>
c) \(f(x) = (x^2 - 1)^2 \cdot (x + 5)^3\) 

<|ref|>equation<|/ref|><|det|>[[263, 475, 600, 505]]<|/det|>
\[
2(x^2-1) \cdot 2x \quad 3(x+5)^2 \cdot 1
\]

<|ref|>equation<|/ref|><|det|>[[183, 517, 744, 560]]<|/det|>
\[
f'(x) = 4x(x^2-1) \cdot (x+5)^3 + (x^2-1)^2 \cdot 3(x+5)^2 \\
= (x^2-1)(x+5)^2 \cdot [4x \cdot (x+5) + 3 \cdot (x^2-1)]
\]

<|ref|>equation<|/ref|><|det|>[[263, 593, 758, 625]]<|/det|>
\[
= (x^2-1)(x+5)^2 \cdot [4x^2 + 20x + 3x^2 - 3]
\]

<|ref|>equation<|/ref|><|det|>[[263, 630, 700, 662]]<|/det|>
\[
= (x^2-1)(x+5)^2 \quad [7x^2 + 20x - 3]
\]