<|ref|>sub_title<|/ref|><|det|>[[20, 8, 551, 40]]<|/det|>
Ableitung der Umkehrungfunktion : 

<|ref|>text<|/ref|><|det|>[[45, 48, 644, 80]]<|/det|>
f : \(\mathbb{R} \to \mathbb{R}\) sei differenzierbar und bijektiv 

<|ref|>text<|/ref|><|det|>[[45, 83, 580, 123]]<|/det|>
Es gilt : \(f^{-1}(y)' = \frac{1}{f'(x)} = \frac{1}{f'(f^{-1}(y))}\) 

<|ref|>text<|/ref|><|det|>[[20, 145, 999, 178]]<|/det|>
Bsp : \(f(x) = (x^2 - x + 1)^4\) \(g(h) = h^4\) \(g'(h) = 4h^3\) 

<|ref|>equation<|/ref|><|det|>[[163, 180, 999, 213]]<|/det|>
\[h(x) = x^2 - x + 1 \quad h'(x) = 2x - 1\]

<|ref|>equation<|/ref|><|det|>[[163, 220, 570, 255]]<|/det|>
\[f'(x) = 4(x^2 - x + 1)^3 \cdot (2x - 1)\]

<|ref|>equation<|/ref|><|det|>[[135, 280, 327, 315]]<|/det|>
\[f(x) = \frac{x}{x^2 + 3}\]

<|ref|>equation<|/ref|><|det|>[[163, 315, 825, 356]]<|/det|>
\[f'(x) = \frac{1 \cdot (x^2 + 3) - x \cdot 2x}{(x^2 + 3)^2} = \frac{x^2 + 3 - 2x^2}{(x^2 + 3)^2} = \frac{-x^2 + 3}{(x^2 + 3)^2}\]