<|ref|>equation<|/ref|><|det|>[[118, 80, 760, 245]]<|/det|>
\[
\begin{align*}
c &= \frac{\sum_{1}^{4} u_i v_i - 4 \bar{u} \bar{v}}{\sum_{1}^{4} u_i^2 - 4 \bar{u}^2} = \frac{-0,313 \cdot 933 - 4 \cdot 1,5 \cdot 0,480 \cdot 832}{14 - 4 \cdot 1,5^2} = -0,639 \cdot 785 \\
d &= \bar{v} - c \bar{u} = 0,480 \cdot 832 - (-0,639 \cdot 785) \cdot 1,5 = 1,440 \cdot 510 \\
\ln a &= d \quad \Rightarrow \quad a = e^d = e^{1,440 \cdot 510} = 4,2229; \quad b = c = -0,6398
\end{align*}
\]

<|ref|>text<|/ref|><|det|>[[118, 228, 465, 246]]<|/det|>
Ausgleichskurve: \(y = 4,2229 \cdot e^{-0,6398x}\)