<|ref|>text<|/ref|><|det|>[[20, 6, 844, 47]]<|/det|>
3) a) \(\langle \vec{e} \times (\vec{b} + \vec{a}), \vec{b} \times \vec{a} - \vec{a} \rangle\) f√ºr \(\vec{a}\) \(\vec{b}\) 

<|ref|>equation<|/ref|><|det|>[[128, 45, 590, 99]]<|/det|>
\[= \langle \vec{e} \times \vec{b} + \vec{e} \times \vec{e}, \vec{b} \times \vec{a} - \vec{a} \rangle\]

<|ref|>equation<|/ref|><|det|>[[128, 100, 500, 135]]<|/det|>
\[= \langle \vec{e} \times \vec{b}, \vec{b} \times \vec{a} - \vec{a} \rangle\]

equation<|/ref|><|det|>[[128, 140, 650, 220]]<|/det|>
\[= \langle \vec{e} \times \vec{b}, \vec{a} \times \vec{a} \rangle - \langle \vec{e} \times \vec{b}, \vec{a} \rangle\]

<|ref|>equation<|/ref|><|det|>[[128, 220, 960, 270]]<|/det|>
\[= - \langle \vec{e} \times \vec{b}, \vec{a} \times \hat{b} \rangle\]

<|ref|>equation<|/ref|><|det|>[[128, 263, 942, 310]]<|/det|>
\[= - \langle \vec{a} \times \vec{b}, \vec{a} \times \hat{b} \rangle = (\sqrt{v_1^2 + \ldots + v_n^2})\]

<|ref|>equation<|/ref|><|det|>[[128, 301, 808, 345]]<|/det|>
\[= - \vec{a} \times \vec{b} \cdot \vec{a} \times \hat{b} \cdot \vec{b} \times \hat{b} \cdot \vec{a} \times \hat{b} \cdot \vec{b}\]

<|ref|>equation<|/ref|><|det|>[[128, 338, 465, 380]]<|/det|>
\[= - \vec{a} \times \vec{b} \cdot \hat{b} \cdot \vec{a} \times \hat{b} \cdot \hat{b} \cdot \vec{a} \times \hat{b}\]

<|ref|>equation<|/ref|><|det|>[[128, 373, 707, 444]]<|/det|>
\[= - \vec{a} \times \vec{b} \cdot \left( \vec{a} \times \hat{b} \right) \cdot \sin\left(4(\vec{a}, \vec{b})\right)^2\]

<|ref|>equation<|/ref|><|det|>[[128, 437, 312, 470]]<|/det|>
\[= - \vec{a} \times \vec{b} \cdot \text{|\vec{b}|}\]

<|ref|>text<|/ref|><|det|>[[77, 515, 572, 550]]<|/det|>
b) \(E: 3x - 6y + 2z - 14 = 0\) 

<|ref|>equation<|/ref|><|det|>[[188, 560, 785, 644]]<|/det|>
\[\vec{n} = \left( \frac{3}{2} \right) \quad |\vec{n}| = \sqrt{3^2 + (-6)^2 + 2^2} = 7\]

<|ref|>equation<|/ref|><|det|>[[140, 666, 944, 755]]<|/det|>
\[\frac{1}{4} \cdot (3x - 6y + 2z - 14) = 0 \quad \text{Hesse Normform}\]

<|ref|>equation<|/ref|><|det|>[[140, 753, 626, 777]]<|/det|>
\[\frac{1}{4} \cdot (3x - 6y) + 2z - \frac{1}{2} = 0\]

<|ref|>text<|/ref|><|det|>[[140, 771, 625, 805]]<|/det|>
d ist der Abstand vom Wurpfung 

<|ref|>equation<|/ref|><|det|>[[140, 828, 737, 897]]<|/det|>
\[E \text{ in Normform} : \langle \vec{n}, \vec{r} \rangle - \langle \vec{n}, \vec{r}_0 \rangle = 0\]

<|ref|>equation<|/ref|><|det|>[[140, 904, 833, 966]]<|/det|>
\[E \text{ in Hesse Normform} : \langle \hat{n}, \vec{r} \rangle - \langle \hat{n}, \vec{r}_0 \rangle = 0\]