<|ref|>text<|/ref|><|det|>[[30, 15, 490, 45]]<|/det|>
4) c) \(\sin(4x) \cdot y + 3y' + \sqrt{x} = 0\) 

<|ref|>equation<|/ref|><|det|>[[144, 52, 465, 84]]<|/det|>
\[3y' = -y \cdot \sin(4x) - \sqrt{x}\]

<|ref|>equation<|/ref|><|det|>[[164, 88, 910, 147]]<|/det|>
\[y' = -y \cdot \frac{1}{3} \sin(4x) - \frac{1}{3} \sqrt{x} \quad \Rightarrow \quad \text{linear & inhomogen}\]

<|ref|>equation<|/ref|><|det|>[[111, 168, 320, 198]]<|/det|>
\[\cdot y'y + x = 0\]

<|ref|>equation<|/ref|><|det|>[[144, 202, 610, 240]]<|/det|>
\[y' = -\frac{x}{y} \quad \Rightarrow \quad \text{nichu linear}\]

<|ref|>equation<|/ref|><|det|>[[111, 263, 360, 293]]<|/det|>
\[\cdot mv + kv = mg\]

<|ref|>equation<|/ref|><|det|>[[144, 295, 840, 353]]<|/det|>
\[\dot{v} = \frac{q}{m} - \frac{k}{m} v \quad \Rightarrow \quad \text{linear, inhomogen, konstante Weyl-Fizienken}\]

<|ref|>equation<|/ref|><|det|>[[111, 371, 370, 410]]<|/det|>
\[\cdot \dot{y} + \frac{1}{t^2} y = e^{3t}\]

<|ref|>equation<|/ref|><|det|>[[144, 412, 760, 475]]<|/det|>
\[\dot{y} = -\frac{1}{t^2} y + e^{3t} \quad \Rightarrow \quad \text{linear, inhomogen}\]