<|ref|>text<|/ref|><|det|>[[111, 16, 546, 45]]<|/det|>
stationäre dösung : \(u' = 0 = 2 - u\) 

<|ref|>equation<|/ref|><|det|>[[381, 58, 465, 80]]<|/det|>
\(u = 2\)

<|ref|>text<|/ref|><|det|>[[111, 92, 615, 123]]<|/det|>
⇒ allgemeine dösung : \(u(x) = 2 + K \cdot e^{-x}\) 

<|ref|>equation<|/ref|><|det|>[[671, 99, 743, 120]]<|/det|>
\(K \in \mathbb{R}\)

<|ref|>text<|/ref|><|det|>[[111, 133, 631, 159]]<|/det|>
Rücksubstitution : \(2x - y = u = 2 + K \cdot e^{-x}\) 

<|ref|>equation<|/ref|><|det|>[[348, 170, 576, 196]]<|/det|>
\(y = 2x - 2 - K \cdot e^{-x}\)