a) Wir modifizieren den Code.
\# Parameter:
$f=5 * *(x * * 3-s p . s q r t(x)+7)$;
Gemäss Ausgabe erhalten wir die Ableitung
$f^{\prime}(x)=\frac{5^{-\sqrt{x}+x^{3}+7} \cdot\left(6 \cdot x^{\frac{5}{2}}-1\right) \cdot \ln (5)}{2 \cdot \sqrt{x}}$.
b) Wir modifizieren den Code.
\# Parameter:
$f=\operatorname{sp} \cdot \log (9 * x * * 2-4,2)$;
Gemäss Ausgabe erhalten wir die Ableitung
$f^{\prime}(x)=\frac{18 \cdot x}{\left(9 \cdot x^{2}-4\right) \cdot \ln (2)}$.
c) Wir modifizieren den Code.
\# Parameter:
$f=($ sp. $\log (x * * 256)) * *(1 / 4)$;
Gemäss Ausgabe erhalten wir die Ableitung
$f^{\prime}(x)=\frac{64.0}{x \cdot \ln ^{0.75}\left(x^{256}\right)}$.
d) Wir modifizieren den Code.
\# Parameter:
$f=1 /(1+\operatorname{sp} \cdot \exp (-x))$;
Gemäss Ausgabe erhalten wir die Ableitung
$f^{\prime}(x)=\frac{1}{4 \cdot \cosh ^{2}\left(\frac{x}{2}\right)}$.
e) Wir modifizieren den Code.
\# Parameter:
$f=($ sp. $\log (x)) * * \operatorname{sp} \cdot \log (x)$;
Gemäss Ausgabe erhalten wir die Ableitung
$f^{\prime}(x)=\frac{(\ln (\ln (x))+1) \cdot \ln ^{\ln (x)}(x)}{x}$.
f) Wir modifizieren den Code.
\# Parameter:
$f=2 * *(-\operatorname{sp.sqrt}(\operatorname{sp} \cdot \operatorname{Abs}(x))) / \operatorname{sp} \cdot \log (2)$;
$f^{\prime}(x)=\left\{\left.\begin{array}{c|c} 

$$
\begin{array}{c}
0 \\
-\frac{2^{-\sqrt{|x|}-1} \cdot x}{\left|x^{\frac{3}{2}}\right|} \\
\hline
\end{array} \right\rvert\, \begin{array}{l}
\text { sonst. }
\end{array}\right.$