<|ref|>text<|/ref|><|det|>[[24, 6, 860, 45]]<|/det|>
2) notare le che exponentiationum f(x) = e^x 

<|ref|>text<|/ref|><|det|>[[78, 45, 625, 84]]<|/det|>
a) exp(0) = 1 ⇒ e^0 = 1 

<|ref|>text<|/ref|><|det|>[[78, 81, 707, 122]]<|/det|>
b) exp"(x) = (e^x)" ⇒ e^x = e^x 

<|ref|>text<|/ref|><|det|>[[78, 120, 830, 161]]<|/det|>
c) exp(0,25) = e^{0,25} = e^{1/2} = e^{0.5} = e^{√e} 

<|ref|>text<|/ref|><|det|>[[78, 160, 920, 201]]<|/det|>
d) exp(2x) = e^{2x} = e^x. e^x ≠ 2. exp(x) = 2. e^x 

<|ref|>text<|/ref|><|det|>[[78, 199, 700, 241]]<|/det|>
e) exp(x-y) = e^{x-y} = e^{x-y} = exp(x-y) 

<|ref|>text<|/ref|><|det|>[[78, 240, 970, 315]]<|/det|>
f) eigenliche exponentiationum: f(x) = a^x, a > 0 für 0 < a < 1: f(x) ist streng monoton fallend 

<|ref|>text<|/ref|><|det|>[[24, 360, 365, 397]]<|/det|>
3) a) sqn(10;π) 

<|ref|>text<|/ref|><|det|>[[450, 365, 777, 433]]<|/det|>
x → sqn(x) = { -1, x < 0
0, x = 0
1, x > 0 

<|ref|>text<|/ref|><|det|>[[157, 455, 880, 491]]<|/det|>
→ alle welle > 0 ⇒ sqn(10;π) = {1} 

<|ref|>text<|/ref|><|det|>[[78, 515, 625, 560]]<|/det|>
b) an = 2n-5-4n² / 3-8n²-10n lim n→∞ an 

<|ref|>text<|/ref|><|det|>[[157, 576, 625, 640]]<|/det|>
lim n→∞ n² (2n-5-4n² / 3-8-10n) = lim n→∞ n² (2n-5-4n² / 3-8-1n) / 0 = lim n→∞ n² (2n-5-4n² / 3-7n) / 0 = lim n→∞ n² (2n-5-4n) / 3n = lim n→∞ n² (2n-5) / 3n = lim n→∞ n² (2n-5) / 2n = lim n→∞ n² (2n-5) / 2n = lim (n→∞) n² (2n-5) / 2n = lim (n→∞) n (2n-5) / 2n = lim (n→∞) n² (n-5) / 2n = lim (n→∞) n² (n-1) / 2n = lim (n→∞) n² (n-1) / n = lim (n→∞) n² (n-1) / n = lim (n→0) n² (n-1) / n = lim (n→0) n² / n = lim (n→0) n² / n = lim (n→0)

<|ref|>text<|/ref|><|det|>[[78, 648, 640, 690]]<|/det|>
c) f'(x) = √3x² + 3²x = (3x² + 3²x)¹/² 

<|ref|>text<|/ref|><|det|>[[137, 688, 844, 770]]<|/det|>
f'(x) = 1/2. (3x² + 3²x)⁻¹/² . (6x + 2.3²x. ln3)
= 6x + 2.3²x. ln3 / 2. √3x² + 3²x¹/² = 2. (3x² + 3²x. ln3) / 2. √3x² + 3²x¹/² = 3x² + 3²x. ln3 / 3x² + 3²x¹/² 

<|ref|>text<|/ref|><|det|>[[78, 784, 900, 900]]<|/det|>
d) -1/2 (2wu - 6vw² + 1) dw = [w²u - 2vw³ + w]⁻¹u
= (-v)²u - 2v(-v)³ - v - u²u + 2vu³ - u
= uv² + 2v4 - v - u³ + 2vu³ - u