$$
\begin{aligned}
& =T_{0}+2 T_{0} \lim _{n \rightarrow \infty} \sum_{k=1}^{n}\left(\frac{2}{3}\right)^{k}=T_{0}+2 T_{0} \lim _{n \rightarrow \infty} G_{(1 ; n)}\left(\frac{2}{3}\right)=T_{0}+2 T_{0} \lim _{n \rightarrow \infty} \frac{\frac{2}{3}-\left(\frac{2}{3}\right)^{n+1}}{1-\frac{2}{3}} \\
& =T_{0}+2 T_{0} \cdot \frac{\frac{2}{3}-0}{1-\frac{2}{3}}=T_{0}+2 T_{0} \cdot \frac{\frac{2}{3}}{\frac{1}{3}}=T_{0}+2 T_{0} \cdot \frac{2}{3} \cdot 3=T_{0}(1+4)=5 T_{0} \\
& =5 \sqrt{\frac{2 H_{0}}{g}} \approx 5 \cdot \sqrt{\frac{2 \cdot 20 \mathrm{~m}}{10 \frac{\mathrm{~m}}{\mathrm{~s}^{2}}}}=5 \cdot \sqrt{4.0 \mathrm{~s}^{2}}=5 \cdot 2.0 \mathrm{~s}=\underline{10 \mathrm{~s}}
\end{aligned}
$$

Der Basketball springt also in der endlichen Zeit $\Delta t$ unendlich viele Male vom Boden auf und f√§llt wieder hinunter!